New version with normal form proof (at last)

thys/NormByEval/NBE.thy
@@ -1,4 +1,4 @@
-(*  ID:         $Id: NBE.thy,v 1.9 2008-10-27 17:45:37 ballarin Exp $
+(*  ID:         $Id: NBE.thy,v 1.10 2009-06-12 06:15:26 nipkow Exp $
     Author:     Klaus Aehlig, Tobias Nipkow
     Normalization by Evaluation
 *)
@@ -8,19 +8,14 @@ theory NBE imports Main begin
 ML"Syntax.ambiguity_level := 1000000"
 
 declare Let_def[simp]
-
-(* still needed for termination proofs: *)
-lemma [simp]: "x \<in> set vs \<Longrightarrow> size x < Suc (list_size size vs)"
-by (induct vs) auto
-lemma [simp]:"x \<in> set vs \<Longrightarrow> size x < Suc (size v + list_size size vs)"
-by (induct vs) auto
 (*>*)
 section "Terms"
 
 types vname = nat
       ml_vname = nat
 
-typedecl cname
+(* FIXME only for codegen*)
+types cname=int
 
 text{* ML terms: *}
 
@@ -63,14 +58,23 @@ Lam: "pure t \<Longrightarrow> pure(\<Lambda> t)" |
 "pure s \<Longrightarrow> pure t \<Longrightarrow> pure(s\<bullet>t)"
 
 declare pure.intros[simp]
+declare Lam[simp del]
+
+lemma pure_Lam[simp]: "pure(\<Lambda> t) = pure t"
+proof
+  assume "pure(\<Lambda> t)" thus "pure t"
+  proof cases qed auto
+next
+  assume "pure t" thus "pure(\<Lambda> t)" by(rule Lam)
+qed
 
 text{* Closed terms w.r.t.\ ML variables:*}
 
 fun closed_ML :: "nat \<Rightarrow> ml \<Rightarrow> bool" ("closed\<^bsub>ML\<^esub>") where
-"closed\<^bsub>ML\<^esub> i (C_ML nm) = True" |
-"closed\<^bsub>ML\<^esub> i (V_ML X) = (X<i)"  |
-"closed\<^bsub>ML\<^esub> i (A_ML v vs) = (closed\<^bsub>ML\<^esub> i v \<and> (\<forall>v \<in> set vs. closed\<^bsub>ML\<^esub> i v))" |
-"closed\<^bsub>ML\<^esub> i (Lam_ML v) = closed\<^bsub>ML\<^esub> (i+1) v" |
+"closed\<^bsub>ML\<^esub> i (C\<^bsub>ML\<^esub> nm) = True" |
+"closed\<^bsub>ML\<^esub> i (V\<^bsub>ML\<^esub> X) = (X<i)"  |
+"closed\<^bsub>ML\<^esub> i (A\<^bsub>ML\<^esub> v vs) = (closed\<^bsub>ML\<^esub> i v \<and> (\<forall>v \<in> set vs. closed\<^bsub>ML\<^esub> i v))" |
+"closed\<^bsub>ML\<^esub> i (Lam\<^bsub>ML\<^esub> v) = closed\<^bsub>ML\<^esub> (i+1) v" |
 "closed\<^bsub>ML\<^esub> i (C\<^isub>U nm vs) = (\<forall>v \<in> set vs. closed\<^bsub>ML\<^esub> i v)" |
 "closed\<^bsub>ML\<^esub> i (V\<^isub>U nm vs) = (\<forall>v \<in> set vs. closed\<^bsub>ML\<^esub> i v)" |
 "closed\<^bsub>ML\<^esub> i (Clo f vs n) = (closed\<^bsub>ML\<^esub> i f \<and> (\<forall>v \<in> set vs. closed\<^bsub>ML\<^esub> i v))" |
@@ -79,8 +83,27 @@ fun closed_ML :: "nat \<Rightarrow> ml \<Rightarrow> bool" ("closed\<^bsub>ML\<^
 fun closed_tm_ML :: "nat \<Rightarrow> tm \<Rightarrow> bool" ("closed\<^bsub>ML\<^esub>") where
 "closed_tm_ML i (r\<bullet>s) = (closed_tm_ML i r \<and> closed_tm_ML i s)" |
 "closed_tm_ML i (\<Lambda> t) = (closed_tm_ML i t)" |
-"closed_tm_ML i (term v) = closed\<^bsub>ML\<^esub> i v" |
+"closed_tm_ML i (term v) = closed_ML i v" |
 "closed_tm_ML i v = True"
+
+text{* Free variables: *}
+
+fun fv_ML :: "ml \<Rightarrow> ml_vname set" ("fv\<^bsub>ML\<^esub>") where
+"fv\<^bsub>ML\<^esub> (C\<^bsub>ML\<^esub> nm) = {}" |
+"fv\<^bsub>ML\<^esub> (V\<^bsub>ML\<^esub> X) = {X}"  |
+"fv\<^bsub>ML\<^esub> (A\<^bsub>ML\<^esub> v vs) = fv\<^bsub>ML\<^esub> v \<union> (\<Union>v \<in> set vs. fv\<^bsub>ML\<^esub> v)" |
+"fv\<^bsub>ML\<^esub> (Lam\<^bsub>ML\<^esub> v) = {X. Suc X : fv\<^bsub>ML\<^esub> v}" |
+"fv\<^bsub>ML\<^esub> (C\<^isub>U nm vs) = (\<Union>v \<in> set vs. fv\<^bsub>ML\<^esub> v)" |
+"fv\<^bsub>ML\<^esub> (V\<^isub>U nm vs) = (\<Union>v \<in> set vs. fv\<^bsub>ML\<^esub> v)" |
+"fv\<^bsub>ML\<^esub> (Clo f vs n) = fv\<^bsub>ML\<^esub> f \<union> (\<Union>v \<in> set vs. fv\<^bsub>ML\<^esub> v)" |
+"fv\<^bsub>ML\<^esub> (apply v w) = fv\<^bsub>ML\<^esub> v \<union> fv\<^bsub>ML\<^esub> w"
+
+primrec fv :: "tm \<Rightarrow> vname set" where
+"fv (C nm) = {}" |
+"fv (V X) = {X}"  |
+"fv (s \<bullet> t) = fv s \<union> fv t" |
+"fv (\<Lambda> t) = {X. Suc X : fv t}"
+
 
 subsection "Iterated Term Application"
 
@@ -118,13 +141,113 @@ apply(rule)
 apply(blast dest:foldl_At_eq_lemma foldl_At_eq_length)
 done
 
+lemma term_eq_foldl_At[simp]:
+  "term v = t \<bullet>\<bullet> ts \<longleftrightarrow> t = term v \<and> ts = []"
+by (induct ts arbitrary:t) auto
+
+lemma At_eq_foldl_At[simp]:
+  "r \<bullet> s = t \<bullet>\<bullet> ts \<longleftrightarrow>
+  (if ts=[] then t = r \<bullet> s else s = last ts \<and> r = t \<bullet>\<bullet> butlast ts)"
+apply (induct ts arbitrary:t)
+ apply fastsimp
+apply rule
+ apply clarsimp
+ apply rule
+  apply clarsimp
+ apply clarsimp
+ apply(subgoal_tac "\<exists>ts' t'. ts = ts' @ [t']")
+  apply clarsimp
+ defer
+ apply (clarsimp split:list.split)
+apply (metis append_butlast_last_id)
+done
+
+lemma foldl_At_eq_At[simp]:
+  "t \<bullet>\<bullet> ts = r \<bullet> s \<longleftrightarrow>
+  (if ts=[] then t = r \<bullet> s else s = last ts \<and> r = t \<bullet>\<bullet> butlast ts)"
+by(metis At_eq_foldl_At)
+
+lemma Lam_eq_foldl_At[simp]:
+  "\<Lambda> s = t \<bullet>\<bullet> ts \<longleftrightarrow> t = \<Lambda> s \<and> ts = []"
+by (induct ts arbitrary:t) auto
+
+lemma foldl_At_eq_Lam[simp]:
+  "t \<bullet>\<bullet> ts = \<Lambda> s \<longleftrightarrow> t = \<Lambda> s \<and> ts = []"
+by (induct ts arbitrary:t) auto
+
+lemma [simp]: "s \<bullet> t \<noteq> s"
+apply(subgoal_tac "size(s \<bullet> t) \<noteq> size s")
+apply metis
+apply simp
+done
+
+(* Better: a simproc for disproving "s = t"
+   if s is a subterm of t or vice versa, by proving "size s ~= size t"
+*)
+
+fun atomic_tm :: "tm \<Rightarrow> bool" where
+"atomic_tm(s \<bullet> t) = False" |
+"atomic_tm(_) = True"
+
+fun head_tm where
+"head_tm(s \<bullet> t) = head_tm s" |
+"head_tm(s) = s"
+
+fun args_tm where
+"args_tm(s \<bullet> t) = args_tm s @ [t]" |
+"args_tm(_) = []"
+
+lemma head_tm_foldl_At[simp]: "head_tm(s \<bullet>\<bullet> ts) = head_tm s"
+by(induct ts arbitrary: s) auto
+
+lemma args_tm_foldl_At[simp]: "args_tm(s \<bullet>\<bullet> ts) = args_tm s @ ts"
+by(induct ts arbitrary: s) auto
+
+lemma tm_eq_iff:
+  "atomic_tm(head_tm s) \<Longrightarrow> atomic_tm(head_tm t)
+   \<Longrightarrow> s = t \<longleftrightarrow> head_tm s = head_tm t \<and> args_tm s = args_tm t"
+apply(induct s arbitrary: t)
+apply(case_tac t, simp+)+
+done
+
+declare
+  tm_eq_iff[of "h \<bullet>\<bullet> ts", standard, simp]
+  tm_eq_iff[of _ "h \<bullet>\<bullet> ts", standard, simp]
+
+lemma atomic_tm_head_tm: "atomic_tm(head_tm t)"
+by(induct t) auto
+
+lemma head_tm_idem: "head_tm(head_tm t) = head_tm t"
+by(induct t) auto
+
+lemma args_tm_head_tm: "args_tm(head_tm t) = []"
+by(induct t) auto
+
+lemma eta_head_args: "t = head_tm t \<bullet>\<bullet> args_tm t"
+by (subst tm_eq_iff) (auto simp: atomic_tm_head_tm head_tm_idem args_tm_head_tm)
+
+
+lemma tm_vector_cases:
+  "(\<exists>n ts. t = V n \<bullet>\<bullet> ts) \<or>
+   (\<exists>nm ts. t = C nm \<bullet>\<bullet> ts) \<or>
+   (\<exists>t' ts. t = \<Lambda> t' \<bullet>\<bullet> ts) \<or>
+   (\<exists>v ts. t = term v \<bullet>\<bullet> ts)"
+apply(induct t)
+apply simp_all
+apply (metis butlast_snoc last_snoc list.simps(1) rotate1_is_Nil_conv rotate_simps)
+done
+
+lemma fv_head_C[simp]: "fv (t \<bullet>\<bullet> ts) = fv t \<union> (\<Union>t\<in>set ts. fv t)"
+by(induct ts arbitrary:t) auto
+
+
 subsection "Lifting and Substitution"
 
 fun lift_ml :: "nat \<Rightarrow> ml \<Rightarrow> ml" ("lift") where
-"lift i (C_ML nm) = C_ML nm" |
-"lift i (V_ML X) = V_ML X" |
-"lift i (A_ML v vs) = A_ML (lift i v) (map (lift i) vs)" |
-"lift i (Lam_ML v) = Lam_ML (lift i v)" |
+"lift i (C\<^bsub>ML\<^esub> nm) = C\<^bsub>ML\<^esub> nm" |
+"lift i (V\<^bsub>ML\<^esub> X) = V\<^bsub>ML\<^esub> X" |
+"lift i (A\<^bsub>ML\<^esub> v vs) = A\<^bsub>ML\<^esub> (lift i v) (map (lift i) vs)" |
+"lift i (Lam\<^bsub>ML\<^esub> v) = Lam\<^bsub>ML\<^esub> (lift i v)" |
 "lift i (C\<^isub>U nm vs) = C\<^isub>U nm (map (lift i) vs)" |
 "lift i (V\<^isub>U x vs) = V\<^isub>U (if x < i then x else x+1) (map (lift i) vs)" |
 "lift i (Clo v vs n) = Clo (lift i v) (map (lift i) vs) n" |
@@ -140,10 +263,10 @@ fun lift_tm :: "nat \<Rightarrow> tm \<Rightarrow> tm" ("lift") where
 "lift i (term v) = term (lift i v)"
 
 fun lift_ML :: "nat \<Rightarrow> ml \<Rightarrow> ml" ("lift\<^bsub>ML\<^esub>") where
-"lift\<^bsub>ML\<^esub> i (C_ML nm) = C_ML nm" |
-"lift\<^bsub>ML\<^esub> i (V_ML X) = V_ML (if X < i then X else X+1)" |
-"lift\<^bsub>ML\<^esub> i (A_ML v vs) = A_ML (lift\<^bsub>ML\<^esub> i v) (map (lift\<^bsub>ML\<^esub> i) vs)" |
-"lift\<^bsub>ML\<^esub> i (Lam_ML v) = Lam_ML (lift\<^bsub>ML\<^esub> (i+1) v)" |
+"lift\<^bsub>ML\<^esub> i (C\<^bsub>ML\<^esub> nm) = C\<^bsub>ML\<^esub> nm" |
+"lift\<^bsub>ML\<^esub> i (V\<^bsub>ML\<^esub> X) = V\<^bsub>ML\<^esub> (if X < i then X else X+1)" |
+"lift\<^bsub>ML\<^esub> i (A\<^bsub>ML\<^esub> v vs) = A\<^bsub>ML\<^esub> (lift\<^bsub>ML\<^esub> i v) (map (lift\<^bsub>ML\<^esub> i) vs)" |
+"lift\<^bsub>ML\<^esub> i (Lam\<^bsub>ML\<^esub> v) = Lam\<^bsub>ML\<^esub> (lift\<^bsub>ML\<^esub> (i+1) v)" |
 "lift\<^bsub>ML\<^esub> i (C\<^isub>U nm vs) = C\<^isub>U nm (map (lift\<^bsub>ML\<^esub> i) vs)" |
 "lift\<^bsub>ML\<^esub> i (V\<^isub>U x vs) = V\<^isub>U x (map (lift\<^bsub>ML\<^esub> i) vs)" |
 "lift\<^bsub>ML\<^esub> i (Clo v vs n) = Clo (lift\<^bsub>ML\<^esub> i v) (map (lift\<^bsub>ML\<^esub> i) vs) n" |
@@ -166,10 +289,10 @@ where
 | "subst \<sigma> (s\<bullet>t) = (subst \<sigma> s) \<bullet> (subst \<sigma> t)"
 
 fun subst_ML :: "(nat \<Rightarrow> ml) \<Rightarrow> ml \<Rightarrow> ml" ("subst\<^bsub>ML\<^esub>") where
-"subst\<^bsub>ML\<^esub> \<sigma> (C_ML nm) = C_ML nm" |
-"subst\<^bsub>ML\<^esub> \<sigma> (V_ML X) = \<sigma> X" |
-"subst\<^bsub>ML\<^esub> \<sigma> (A_ML v vs) = A_ML (subst\<^bsub>ML\<^esub> \<sigma> v) (map (subst\<^bsub>ML\<^esub> \<sigma>) vs)" |
-"subst\<^bsub>ML\<^esub> \<sigma> (Lam_ML v) = Lam_ML (subst\<^bsub>ML\<^esub> (V_ML 0 ## \<sigma>) v)" |
+"subst\<^bsub>ML\<^esub> \<sigma> (C\<^bsub>ML\<^esub> nm) = C\<^bsub>ML\<^esub> nm" |
+"subst\<^bsub>ML\<^esub> \<sigma> (V\<^bsub>ML\<^esub> X) = \<sigma> X" |
+"subst\<^bsub>ML\<^esub> \<sigma> (A\<^bsub>ML\<^esub> v vs) = A\<^bsub>ML\<^esub> (subst\<^bsub>ML\<^esub> \<sigma> v) (map (subst\<^bsub>ML\<^esub> \<sigma>) vs)" |
+"subst\<^bsub>ML\<^esub> \<sigma> (Lam\<^bsub>ML\<^esub> v) = Lam\<^bsub>ML\<^esub> (subst\<^bsub>ML\<^esub> (V\<^bsub>ML\<^esub> 0 ## \<sigma>) v)" |
 "subst\<^bsub>ML\<^esub> \<sigma> (C\<^isub>U nm vs) = C\<^isub>U nm (map (subst\<^bsub>ML\<^esub> \<sigma>) vs)" |
 "subst\<^bsub>ML\<^esub> \<sigma> (V\<^isub>U x vs) = V\<^isub>U x (map (subst\<^bsub>ML\<^esub> \<sigma>) vs)" |
 "subst\<^bsub>ML\<^esub> \<sigma> (Clo v vs n) = Clo (subst\<^bsub>ML\<^esub> \<sigma> v) (map (subst\<^bsub>ML\<^esub> \<sigma>) vs) n" |
@@ -180,16 +303,24 @@ lemmas [code] = subst_ML.simps *)
 
 abbreviation
   subst_decr :: "nat \<Rightarrow> tm \<Rightarrow> nat \<Rightarrow> tm" where
- "subst_decr k t \<equiv> \<lambda>n. if n<k then V n else if n=k then t else V(n - 1)"
+  "subst_decr k t \<equiv> \<lambda>n. if n<k then V n else if n=k then t else V(n - 1)"
 abbreviation
   subst_decr_ML :: "nat \<Rightarrow> ml \<Rightarrow> nat \<Rightarrow> ml" where
- "subst_decr_ML k v \<equiv> \<lambda>n. if n<k then V_ML n else if n=k then v else V_ML(n - 1)"
+"subst_decr_ML k v \<equiv> \<lambda>n. if n<k then V\<^bsub>ML\<^esub> n else if n=k then v else V\<^bsub>ML\<^esub>(n - 1)"
 abbreviation
   subst1 :: "tm \<Rightarrow> tm \<Rightarrow> nat \<Rightarrow> tm" ("(_/[_'/_])" [300, 0, 0] 300) where
  "s[t/k] \<equiv> subst (subst_decr k t) s"
 abbreviation
   subst1_ML :: "ml \<Rightarrow> ml \<Rightarrow> nat \<Rightarrow> ml" ("(_/[_'/_])" [300, 0, 0] 300) where
  "u[v/k] \<equiv> subst\<^bsub>ML\<^esub> (subst_decr_ML k v) u"
+
+lemma apply_cons[simp]:
+  "(t##\<sigma>) i = (if i=0 then t::tm else lift 0 (\<sigma>(i - 1)))"
+by(simp add: cons_def split:nat.split)
+
+lemma apply_cons_ML[simp]:
+  "(v##\<sigma>) i = (if i=0 then v::ml else lift\<^bsub>ML\<^esub> 0 (\<sigma>(i - 1)))"
+by(simp add: cons_ML_def split:nat.split)
 
 lemma lift_foldl_At[simp]:
   "lift k (s \<bullet>\<bullet> ts) = (lift k s) \<bullet>\<bullet> (map (lift k) ts)"
@@ -214,20 +345,16 @@ by(induct v arbitrary: i j rule:lift_ML.induct)
   (simp_all add:map_compose[symmetric])
 
 lemma V_ML_cons_ML_subst_decr[simp]:
-  "V_ML 0 ## subst_decr_ML k v = subst_decr_ML (Suc k) (lift\<^bsub>ML\<^esub> 0 v)"
+  "V\<^bsub>ML\<^esub> 0 ## subst_decr_ML k v = subst_decr_ML (Suc k) (lift\<^bsub>ML\<^esub> 0 v)"
 by(rule ext)(simp add:cons_ML_def split:nat.split)
 
 lemma shift_subst_decr[simp]:
  "V 0 ## subst_decr k t = subst_decr (Suc k) (lift 0 t)"
-apply(rule ext)
-apply(simp add:cons_def split:nat.split)
-done
+by(rule ext)(simp add:cons_def split:nat.split)
 
 lemma lift_comp_subst_decr[simp]:
   "lift 0 o subst_decr_ML k v = subst_decr_ML k (lift 0 v)"
-apply(rule ext)
-apply(simp add:cons_ML_def split:nat.split)
-done
+by(rule ext) simp
 
 lemma subst_ML_ext: "\<forall>i. \<sigma> i = \<sigma>' i \<Longrightarrow> subst\<^bsub>ML\<^esub> \<sigma> v = subst\<^bsub>ML\<^esub> \<sigma>' v"
 by(metis ext)
@@ -238,25 +365,19 @@ by(metis ext)
 lemma lift_Pure_tms[simp]: "pure t \<Longrightarrow> pure(lift k t)"
 by(induct arbitrary:k pred:pure) simp_all
 
-lemma cons_ML_V_ML[simp]: "(V\<^bsub>ML\<^esub> 0 ## V\<^bsub>ML\<^esub>) = V_ML"
-apply(rule ext)
-apply(simp add:cons_ML_def split:nat.split)
-done
+lemma cons_ML_V_ML[simp]: "(V\<^bsub>ML\<^esub> 0 ## V\<^bsub>ML\<^esub>) = V\<^bsub>ML\<^esub>"
+by(rule ext) simp
 
 lemma cons_V[simp]: "(V 0 ## V) = V"
-apply(rule ext)
-apply(simp add:cons_def split:nat.split)
-done
+by(rule ext) simp
 
-lemma lift_o_shift: "lift k \<circ> (V_ML 0 ## \<sigma>) = (V_ML 0 ## (lift k \<circ> \<sigma>))"
-apply(rule ext)
-apply (simp add:cons_ML_def lift_lift_ML_comm split:nat.split)
-done
+lemma lift_o_shift: "lift k \<circ> (V\<^bsub>ML\<^esub> 0 ## \<sigma>) = (V\<^bsub>ML\<^esub> 0 ## (lift k \<circ> \<sigma>))"
+by(rule ext)(simp add: lift_lift_ML_comm)
 
 lemma lift_subst_ML:
  "lift k (subst\<^bsub>ML\<^esub> \<sigma> v) = subst\<^bsub>ML\<^esub> (lift k \<circ> \<sigma>) (lift k v)"
 apply(induct \<sigma> v rule:subst_ML.induct)
-apply(simp_all add:map_compose[symmetric] o_assoc lift_o_shift)
+apply(simp_all add:map_compose[symmetric] o_assoc lift_o_shift del:apply_cons_ML)
 apply(simp add:o_def)
 done
 
@@ -269,44 +390,42 @@ done
 
 lemma lift_ML_subst_ML:
  "lift\<^bsub>ML\<^esub> k (subst\<^bsub>ML\<^esub> \<sigma> v) =
-  subst\<^bsub>ML\<^esub> (\<lambda>i. if i<k then lift\<^bsub>ML\<^esub> k (\<sigma> i) else if i=k then V_ML k else lift\<^bsub>ML\<^esub> k (\<sigma>(i - 1))) (lift\<^bsub>ML\<^esub> k v)"
+  subst\<^bsub>ML\<^esub> (\<lambda>i. if i<k then lift\<^bsub>ML\<^esub> k (\<sigma> i) else if i=k then V\<^bsub>ML\<^esub> k else lift\<^bsub>ML\<^esub> k (\<sigma>(i - 1))) (lift\<^bsub>ML\<^esub> k v)"
   (is "_ = subst\<^bsub>ML\<^esub> (?insrt k \<sigma>) (lift\<^bsub>ML\<^esub> k v)")
 apply (induct k v arbitrary: \<sigma> k rule: lift_ML.induct)
 apply (simp_all add:map_compose[symmetric] o_assoc lift_o_shift)
-apply(subgoal_tac "V_ML 0 ## ?insrt k \<sigma> = ?insrt (Suc k) (V_ML 0 ## \<sigma>)")
+apply(subgoal_tac "V\<^bsub>ML\<^esub> 0 ## ?insrt k \<sigma> = ?insrt (Suc k) (V\<^bsub>ML\<^esub> 0 ## \<sigma>)")
  apply simp
 apply (simp add:expand_fun_eq lift_lift_ML cons_ML_def split:nat.split)
 done
 
 corollary subst_cons_lift:
- "subst\<^bsub>ML\<^esub> (V_ML 0 ## \<sigma>) o (lift\<^bsub>ML\<^esub> 0) = lift\<^bsub>ML\<^esub> 0 o (subst\<^bsub>ML\<^esub> \<sigma>)"
+ "subst\<^bsub>ML\<^esub> (V\<^bsub>ML\<^esub> 0 ## \<sigma>) o (lift\<^bsub>ML\<^esub> 0) = lift\<^bsub>ML\<^esub> 0 o (subst\<^bsub>ML\<^esub> \<sigma>)"
 apply(rule ext)
-apply(simp add: cons_ML_def lift_ML_subst_ML)
-apply(subgoal_tac "nat_case (V_ML 0) (\<lambda>j. lift\<^bsub>ML\<^esub> 0 (\<sigma> j)) = (\<lambda>i. if i = 0 then V_ML 0 else lift\<^bsub>ML\<^esub> 0 (\<sigma> (i - 1)))")
+apply(simp add: lift_ML_subst_ML)
+apply(subgoal_tac "(V\<^bsub>ML\<^esub> 0 ## \<sigma>) = (\<lambda>i. if i = 0 then V\<^bsub>ML\<^esub> 0 else lift\<^bsub>ML\<^esub> 0 (\<sigma> (i - 1)))")
  apply simp
-apply(rule ext, simp split:nat.split)
+apply(rule ext, simp)
 done
 
 lemma lift_ML_id[simp]: "closed\<^bsub>ML\<^esub> k v \<Longrightarrow> lift\<^bsub>ML\<^esub> k v = v"
 by(induct k v rule: lift_ML.induct)(simp_all add:list_eq_iff_nth_eq)
 
 lemma subst_ML_id:
-  "closed\<^bsub>ML\<^esub> k v \<Longrightarrow> \<forall>i<k. \<sigma> i = V_ML i \<Longrightarrow> subst\<^bsub>ML\<^esub> \<sigma> v = v"
+  "closed\<^bsub>ML\<^esub> k v \<Longrightarrow> \<forall>i<k. \<sigma> i = V\<^bsub>ML\<^esub> i \<Longrightarrow> subst\<^bsub>ML\<^esub> \<sigma> v = v"
 apply (induct \<sigma> v arbitrary: k rule: subst_ML.induct)
 apply (auto simp add: list_eq_iff_nth_eq)
-    apply(simp add:Ball_def)
-    apply(erule_tac x="vs!i" in meta_allE)
-    apply(erule_tac x="k" in meta_allE)
-    apply(erule_tac x="k" in meta_allE)
-    apply simp
-   apply(erule_tac x="Suc k" in meta_allE)
-   apply (simp add:cons_ML_def split:nat.split)
+   apply(simp add:Ball_def)
    apply(erule_tac x="vs!i" in meta_allE)
+   apply(erule_tac x="k" in meta_allE)
    apply(erule_tac x="k" in meta_allE)
    apply simp
   apply(erule_tac x="vs!i" in meta_allE)
   apply(erule_tac x="k" in meta_allE)
   apply simp
+ apply(erule_tac x="vs!i" in meta_allE)
+ apply(erule_tac x="k" in meta_allE)
+ apply simp
 apply(erule_tac x="vs!i" in meta_allE)
 apply(erule_tac x="k" in meta_allE)
 apply(erule_tac x="k" in meta_allE)
@@ -318,16 +437,15 @@ using subst_ML_id[where k=0] by simp
 
 lemma subst_ML_coincidence:
   "closed\<^bsub>ML\<^esub> k v \<Longrightarrow> \<forall>i<k. \<sigma> i = \<sigma>' i \<Longrightarrow> subst\<^bsub>ML\<^esub> \<sigma> v = subst\<^bsub>ML\<^esub> \<sigma>' v"
-by (induct \<sigma> v arbitrary: k \<sigma>' rule: subst_ML.induct)
-   (auto simp:cons_ML_def split:nat.split)
+by (induct \<sigma> v arbitrary: k \<sigma>' rule: subst_ML.induct) auto
 
 lemma subst_ML_comp:
   "subst\<^bsub>ML\<^esub> \<sigma> (subst\<^bsub>ML\<^esub> \<sigma>' v) = subst\<^bsub>ML\<^esub> (subst\<^bsub>ML\<^esub> \<sigma>  \<circ> \<sigma>') v"
 apply (induct \<sigma>' v arbitrary: \<sigma> rule: subst_ML.induct)
 apply (simp_all add: list_eq_iff_nth_eq)
 apply(rule subst_ML_ext)
-apply(auto simp:cons_ML_def split:nat.split)
-apply (metis cons_ML_def o_apply subst_cons_lift)
+apply simp
+apply (metis o_apply subst_cons_lift)
 done
 
 lemma subst_ML_comp2:
@@ -348,13 +466,11 @@ by (induct k v arbitrary: n rule: lift_ML.induct) simp_all
 
 lemma closed_ML_subst_ML:
   "\<forall>i. closed\<^bsub>ML\<^esub> k (\<sigma> i) \<Longrightarrow> closed\<^bsub>ML\<^esub> k (subst\<^bsub>ML\<^esub> \<sigma> v)"
-by(induct \<sigma> v arbitrary: k rule: subst_ML.induct)
-  (auto simp:cons_ML_def closed_ML_Suc split:nat.split)
+by(induct \<sigma> v arbitrary: k rule: subst_ML.induct) (auto simp: closed_ML_Suc)
 
 lemma closed_ML_subst_ML2:
   "closed\<^bsub>ML\<^esub> k v \<Longrightarrow> \<forall>i<k. closed\<^bsub>ML\<^esub> l (\<sigma> i) \<Longrightarrow> closed\<^bsub>ML\<^esub> l (subst\<^bsub>ML\<^esub> \<sigma> v)"
-by(induct \<sigma> v arbitrary: k l rule: subst_ML.induct)
-  (auto simp:cons_ML_def closed_ML_Suc split:nat.split)
+by(induct \<sigma> v arbitrary: k l rule: subst_ML.induct)(auto simp: closed_ML_Suc)
 
 
 lemma subst_foldl[simp]:
@@ -381,7 +497,7 @@ done
 
 corollary lift_subst:
   "pure t \<Longrightarrow> lift 0 (subst \<sigma> t) = subst (V 0 ## \<sigma>) (lift 0 t)"
-by (simp add: lift_subst_aux cons_def lift_lift_ml split:nat.split)
+by (simp add: lift_subst_aux lift_lift_ml)
 
 lemma subst_comp:
   "pure t \<Longrightarrow> \<forall>i. pure(\<sigma>' i) \<Longrightarrow>
@@ -396,31 +512,64 @@ apply(erule meta_allE)+
 apply(erule meta_impE)
 defer
 apply(erule meta_mp)
-prefer 2 apply (simp add:cons_def split:nat.split)
+prefer 2 apply simp
 apply(rule ext)
-apply(subst (1) cons_def)
-apply(subst (2) cons_def)
-apply(simp split:nat.split)
-apply rule apply (simp add:cons_def)
 apply(simp add:lift_subst)
 done
 
 
 section "Reduction"
 
-text{* Rewrite rules and their compiled version: *}
-axiomatization
-  R :: "(cname * tm list * tm)set"
-consts
-  compR :: "(cname * ml list * ml)set"
+subsection "Patterns"
 
-text{* Reduction of lambda-terms: *}
+inductive pattern :: "tm \<Rightarrow> bool" where
+pat_V: "pattern(V X)" |
+pat_C: "\<forall>t\<in>set ts. pattern t \<Longrightarrow> pattern(C nm \<bullet>\<bullet> ts)"
+
+lemma pattern_Lam[simp]: "\<not> pattern(\<Lambda> t)"
+by(auto elim!: pattern.cases)
+
+lemma pattern_At'D12: "pattern r \<Longrightarrow> r = (s \<bullet> t) \<Longrightarrow> pattern s \<and> pattern t"
+proof(induct arbitrary: s t pred:pattern)
+  case pat_V thus ?case by simp
+next
+  case pat_C thus ?case
+    by (simp add: atomic_tm_head_tm split:split_if_asm)
+       (metis eta_head_args in_set_butlastD pattern.pat_C)
+qed
+
+lemma pattern_AtD12: "pattern(s \<bullet> t) \<Longrightarrow> pattern s \<and> pattern t"
+by(metis pattern_At'D12)
+
+lemma pattern_At_vecD: "pattern(s \<bullet>\<bullet> ts) \<Longrightarrow> \<forall>t \<in> set ts. pattern t"
+apply(induct ts rule:rev_induct)
+ apply simp
+apply (fastsimp dest!:pattern_AtD12)
+done
+
+lemma pattern_At_decomp: "pattern(s \<bullet> t) \<Longrightarrow> \<exists>nm ss. s = C nm \<bullet>\<bullet> ss"
+proof(induct s arbitrary: t)
+  case (At s1 s2) show ?case
+(* FIXME fails using At apply (metis foldl_Cons foldl_Nil foldl_append pattern_AtD1) *)
+    using pattern_AtD12[OF At.prems] At(1)[of s2]
+    by clarsimp (metis append_is_Nil_conv butlast_snoc last_snoc not_Cons_self)
+qed (auto elim!: pattern.cases split:split_if_asm)
+
+
+subsection "Reduction of @{text \<lambda>}-terms"
+
+text{* The source program: *}
+
+axiomatization R :: "(cname * tm list * tm)set" where
+pure_R: "(nm,ts,t) : R \<Longrightarrow> (\<forall>t \<in> set ts. pure t) \<and> pure t" and
+fv_R:   "(nm,ts,t) : R \<Longrightarrow> X : fv t \<Longrightarrow> \<exists>t' \<in> set ts. X : fv t'" and
+pattern_R: "(nm,ts,t') : R \<Longrightarrow> \<forall>t \<in> set ts. pattern t"
 
 inductive_set
-  tRed :: "(tm * tm)set"
-  and tred :: "[tm, tm] => bool"  (infixl "\<rightarrow>" 50)
+  Red_tm :: "(tm * tm)set"
+  and red_tm :: "[tm, tm] => bool"  (infixl "\<rightarrow>" 50)
 where
-  "s \<rightarrow> t \<equiv> (s, t) \<in> tRed"
+  "s \<rightarrow> t \<equiv> (s, t) \<in> Red_tm"
  -- {*$\beta$-reduction*}
 | "(\<Lambda> t) \<bullet> s \<rightarrow> t[s/0]"
  -- {*$\eta$-expansion*}
@@ -432,36 +581,118 @@ where
 | "t \<rightarrow> t' \<Longrightarrow> s \<bullet> t \<rightarrow> s \<bullet> t'"
 
 abbreviation
-  treds :: "[tm, tm] => bool"  (infixl "\<rightarrow>*" 50) where
-  "s \<rightarrow>* t \<equiv> (s, t) \<in> tRed^*"
+  reds_tm :: "[tm, tm] => bool"  (infixl "\<rightarrow>*" 50) where
+  "s \<rightarrow>* t \<equiv> (s, t) \<in> Red_tm^*"
 
 inductive_set
-  tRed_list :: "(tm list * tm list) set"
-  and treds_list :: "[tm list, tm list] \<Rightarrow> bool" (infixl "\<rightarrow>*" 50)
+  Reds_tm_list :: "(tm list * tm list) set"
+  and reds_tm_list :: "[tm list, tm list] \<Rightarrow> bool" (infixl "\<rightarrow>*" 50)
 where
-  "ss \<rightarrow>* ts \<equiv> (ss, ts) \<in> tRed_list"
+  "ss \<rightarrow>* ts \<equiv> (ss, ts) \<in> Reds_tm_list"
 | "[] \<rightarrow>* []"
 | "ts \<rightarrow>* ts' \<Longrightarrow> t \<rightarrow>* t' \<Longrightarrow> t#ts \<rightarrow>* t'#ts'"
 
-text{* Reduction of ML-terms: *}
+
+declare Reds_tm_list.intros[simp]
+
+lemma Reds_tm_list_refl[simp]: fixes ts :: "tm list" shows "ts \<rightarrow>* ts"
+by(induct ts) auto
+
+lemma Red_tm_append: "rs \<rightarrow>* rs' \<Longrightarrow> ts \<rightarrow>* ts' \<Longrightarrow> rs @ ts \<rightarrow>* rs' @ ts'"
+by(induct set: Reds_tm_list) auto
+
+lemma Red_tm_rev: "ts \<rightarrow>* ts' \<Longrightarrow> rev ts \<rightarrow>* rev ts'"
+by(induct set: Reds_tm_list) (auto simp:Red_tm_append)
+
+lemma red_Lam[simp]: "t \<rightarrow>* t' \<Longrightarrow> \<Lambda> t \<rightarrow>* \<Lambda> t'"
+apply(induct rule:rtrancl_induct)
+apply(simp_all)
+apply(blast intro: rtrancl_into_rtrancl Red_tm.intros)
+done
+
+lemma red_At1[simp]: "t \<rightarrow>* t' \<Longrightarrow> t \<bullet> s \<rightarrow>* t' \<bullet> s"
+apply(induct rule:rtrancl_induct)
+apply(simp_all)
+apply(blast intro: rtrancl_into_rtrancl Red_tm.intros)
+done
+
+lemma red_At2[simp]: "t \<rightarrow>* t' \<Longrightarrow> s \<bullet> t \<rightarrow>* s \<bullet> t'"
+apply(induct rule:rtrancl_induct)
+apply(simp_all)
+apply(blast intro:rtrancl_into_rtrancl Red_tm.intros)
+done
+
+lemma Reds_tm_list_foldl_At:
+ "ts \<rightarrow>* ts' \<Longrightarrow> s \<rightarrow>* s' \<Longrightarrow> s \<bullet>\<bullet> ts \<rightarrow>* s' \<bullet>\<bullet> ts'"
+apply(induct arbitrary:s s' rule:Reds_tm_list.induct)
+apply simp
+apply simp
+apply(blast dest: red_At1 red_At2 intro:rtrancl_trans)
+done
+
+
+subsection "Reduction of ML-terms"
+
+text{* The compiled rule set: *}
+
+consts compR :: "(cname * ml list * ml)set"
+
+text{* The actual definition is given later. *}
+
+text{* Now we characterize ML values that cannot possibly be rewritten by a
+rule in @{const compR}. *}
+
+lemma termination_no_match_ML:
+  "i < length ps \<Longrightarrow> rev ps ! i = C\<^isub>U nm vs
+   \<Longrightarrow> listsum (map size vs) < listsum (map size ps)"
+apply(subgoal_tac "C\<^isub>U nm vs : set ps")
+ apply(drule listsum_map_remove1[of _ _ size])
+ apply (simp add:list_size_conv_listsum)
+apply (metis in_set_conv_nth length_rev set_rev)
+done
+
+declare conj_cong[fundef_cong]
+
+function no_match_ML ("no'_match\<^bsub>ML\<^esub>") where
+"no_match\<^bsub>ML\<^esub> ps os =
+  (\<exists>i < min (size os) (size ps).
+   \<exists>nm nm' vs vs'. (rev ps)!i = C\<^isub>U nm vs \<and> (rev os)!i = C\<^isub>U nm' vs' \<and>
+      (nm=nm' \<longrightarrow> no_match\<^bsub>ML\<^esub> vs vs'))"
+by pat_completeness auto
+termination
+apply(relation "measure(%(vs::ml list,_). \<Sum>v\<leftarrow>vs. size v)")
+apply (auto simp:termination_no_match_ML)
+done
+
+
+abbreviation
+"no_match_compR nm os \<equiv>
+  \<forall>(nm',ps,v)\<in> compR. nm=nm' \<longrightarrow> no_match\<^bsub>ML\<^esub> ps os"
+
+declare no_match_ML.simps[simp del]
 
 inductive_set
-  Red :: "(ml * ml)set"
-  and Redl :: "(ml list * ml list)set"
-  and red :: "[ml, ml] => bool"  (infixl "\<Rightarrow>" 50)
-  and redl :: "[ml list, ml list] => bool"  (infixl "\<Rightarrow>" 50)
-  and reds :: "[ml, ml] => bool"  (infixl "\<Rightarrow>*" 50)
+  Red_ml :: "(ml * ml)set"
+  and Red_ml_list :: "(ml list * ml list)set"
+  and red_ml :: "[ml, ml] => bool"  (infixl "\<Rightarrow>" 50)
+  and red_ml_list :: "[ml list, ml list] => bool"  (infixl "\<Rightarrow>" 50)
+  and reds_ml :: "[ml, ml] => bool"  (infixl "\<Rightarrow>*" 50)
 where
-  "s \<Rightarrow> t \<equiv> (s, t) \<in> Red"
-| "s \<Rightarrow> t \<equiv> (s, t) \<in> Redl"
-| "s \<Rightarrow>* t \<equiv> (s, t) \<in> Red^*"
+  "s \<Rightarrow> t \<equiv> (s, t) \<in> Red_ml"
+| "ss \<Rightarrow> ts \<equiv> (ss, ts) \<in> Red_ml_list"
+| "s \<Rightarrow>* t \<equiv> (s, t) \<in> Red_ml^*"
  -- {* ML $\beta$-reduction *}
-| "A_ML (Lam_ML u) [v] \<Rightarrow> u[v/0]"
+| "A\<^bsub>ML\<^esub> (Lam\<^bsub>ML\<^esub> u) [v] \<Rightarrow> u[v/0]"
  -- "Execution of a compiled rewrite rule"
 | "(nm,vs,v) : compR \<Longrightarrow> \<forall> i. closed\<^bsub>ML\<^esub> 0 (\<sigma> i) \<Longrightarrow>
-   A_ML (C_ML nm) (map (subst\<^bsub>ML\<^esub> \<sigma>) vs) \<Rightarrow> subst\<^bsub>ML\<^esub> \<sigma> v"
+   A\<^bsub>ML\<^esub> (C\<^bsub>ML\<^esub> nm) (map (subst\<^bsub>ML\<^esub> \<sigma>) vs) \<Rightarrow> subst\<^bsub>ML\<^esub> \<sigma> v"
+-- {* default rule: *}
+| "\<forall>i. closed\<^bsub>ML\<^esub> 0 (\<sigma> i)
+   \<Longrightarrow> vs = map V\<^bsub>ML\<^esub> [0..<arity nm] \<Longrightarrow> vs' = map (subst\<^bsub>ML\<^esub> \<sigma>) vs
+   \<Longrightarrow> no_match_compR nm vs'
+   \<Longrightarrow> A\<^bsub>ML\<^esub> (C\<^bsub>ML\<^esub> nm) vs' \<Rightarrow> subst\<^bsub>ML\<^esub> \<sigma> (C\<^isub>U nm vs)"
  -- {* Equations for function \texttt{apply}*}
-| apply_Clo1: "apply (Clo f vs (Suc 0)) v \<Rightarrow> A_ML f (v # vs)"
+| apply_Clo1: "apply (Clo f vs (Suc 0)) v \<Rightarrow> A\<^bsub>ML\<^esub> f (v # vs)"
 | apply_Clo2: "n > 0 \<Longrightarrow>
  apply (Clo f vs (Suc n)) v \<Rightarrow> Clo f (v # vs) n"
 | apply_C: "apply (C\<^isub>U nm vs) v \<Rightarrow> C\<^isub>U nm (v # vs)"
@@ -473,18 +704,18 @@ where
 | ctxt_Clo3: "vs \<Rightarrow> vs' \<Longrightarrow> Clo f vs n \<Rightarrow> Clo f vs' n"
 | ctxt_apply1: "s \<Rightarrow> s'   \<Longrightarrow> apply s t \<Rightarrow> apply s' t"
 | ctxt_apply2: "t \<Rightarrow> t'   \<Longrightarrow> apply s t \<Rightarrow> apply s t'"
-| ctxt_A_ML1: "f \<Rightarrow> f'   \<Longrightarrow> A_ML f vs \<Rightarrow> A_ML f' vs"
-| ctxt_A_ML2: "vs \<Rightarrow> vs' \<Longrightarrow> A_ML f vs \<Rightarrow> A_ML f vs'"
+| ctxt_A_ML1: "f \<Rightarrow> f'   \<Longrightarrow> A\<^bsub>ML\<^esub> f vs \<Rightarrow> A\<^bsub>ML\<^esub> f' vs"
+| ctxt_A_ML2: "vs \<Rightarrow> vs' \<Longrightarrow> A\<^bsub>ML\<^esub> f vs \<Rightarrow> A\<^bsub>ML\<^esub> f vs'"
 | ctxt_list1: "v \<Rightarrow> v'   \<Longrightarrow> v#vs \<Rightarrow> v'#vs"
 | ctxt_list2: "vs \<Rightarrow> vs' \<Longrightarrow> v#vs \<Rightarrow> v#vs'"
 
 inductive_set
-  Redt :: "(tm * tm)set"
-  and redt :: "[tm, tm] => bool"  (infixl "\<Rightarrow>" 50)
-  and redts :: "[tm, tm] => bool"  (infixl "\<Rightarrow>*" 50)
+  Red_term :: "(tm * tm)set"
+  and red_term :: "[tm, tm] => bool"  (infixl "\<Rightarrow>" 50)
+  and reds_term :: "[tm, tm] => bool"  (infixl "\<Rightarrow>*" 50)
 where
-  "s \<Rightarrow> t \<equiv> (s, t) \<in> Redt"
-| "s \<Rightarrow>* t \<equiv> (s, t) \<in> Redt^*"
+  "s \<Rightarrow> t \<equiv> (s, t) \<in> Red_term"
+| "s \<Rightarrow>* t \<equiv> (s, t) \<in> Red_term^*"
  --{* function \texttt{term} *}
 | term_C: "term (C\<^isub>U nm vs) \<Rightarrow> (C nm) \<bullet>\<bullet> (map term (rev vs))"
 | term_V: "term (V\<^isub>U x vs) \<Rightarrow> (V x) \<bullet>\<bullet> (map term (rev vs))"
@@ -495,42 +726,6 @@ where
 | ctxt_At2: "t \<Rightarrow> t' \<Longrightarrow> s \<bullet> t \<Rightarrow> s \<bullet> t'"
 | ctxt_term: "v \<Rightarrow> v' \<Longrightarrow> term v \<Rightarrow> term v'"
 
-declare tRed_list.intros[simp]
-
-lemma tRed_list_refl[simp]: fixes ts :: "tm list" shows "ts \<rightarrow>* ts"
-by(induct ts) auto
-
-lemma tRed_append: "rs \<rightarrow>* rs' \<Longrightarrow> ts \<rightarrow>* ts' \<Longrightarrow> rs @ ts \<rightarrow>* rs' @ ts'"
-by(induct set: tRed_list) auto
-
-lemma tRed_rev: "ts \<rightarrow>* ts' \<Longrightarrow> rev ts \<rightarrow>* rev ts'"
-by(induct set: tRed_list) (auto simp:tRed_append)
-
-lemma red_Lam[simp]: "t \<rightarrow>* t' \<Longrightarrow> \<Lambda> t \<rightarrow>* \<Lambda> t'"
-apply(induct rule:rtrancl_induct)
-apply(simp_all)
-apply(blast intro: rtrancl_into_rtrancl tRed.intros)
-done
-
-lemma red_At1[simp]: "t \<rightarrow>* t' \<Longrightarrow> t \<bullet> s \<rightarrow>* t' \<bullet> s"
-apply(induct rule:rtrancl_induct)
-apply(simp_all)
-apply(blast intro: rtrancl_into_rtrancl tRed.intros)
-done
-
-lemma red_At2[simp]: "t \<rightarrow>* t' \<Longrightarrow> s \<bullet> t \<rightarrow>* s \<bullet> t'"
-apply(induct rule:rtrancl_induct)
-apply(simp_all)
-apply(blast intro:rtrancl_into_rtrancl tRed.intros)
-done
-
-lemma tRed_list_foldl_At:
- "ts \<rightarrow>* ts' \<Longrightarrow> s \<rightarrow>* s' \<Longrightarrow> s \<bullet>\<bullet> ts \<rightarrow>* s' \<bullet>\<bullet> ts'"
-apply(induct arbitrary:s s' rule:tRed_list.induct)
-apply simp
-apply simp
-apply(blast dest: red_At1 red_At2 intro:rtrancl_trans)
-done
 
 section "Kernel"
 
@@ -538,10 +733,10 @@ text{* First a special size function and some lemmas for the
 termination proof of the kernel function. *}
 
 fun size' :: "ml \<Rightarrow> nat" where
-"size' (C_ML nm) = 1" |
-"size' (V_ML X) = 1"  |
-"size' (A_ML v vs) = (size' v + (\<Sum>v\<leftarrow>vs. size' v))+1" |
-"size' (Lam_ML v) = size' v + 1" |
+"size' (C\<^bsub>ML\<^esub> nm) = 1" |
+"size' (V\<^bsub>ML\<^esub> X) = 1"  |
+"size' (A\<^bsub>ML\<^esub> v vs) = (size' v + (\<Sum>v\<leftarrow>vs. size' v))+1" |
+"size' (Lam\<^bsub>ML\<^esub> v) = size' v + 1" |
 "size' (C\<^isub>U nm vs) = (\<Sum>v\<leftarrow>vs. size' v)+1" |
 "size' (V\<^isub>U nm vs) = (\<Sum>v\<leftarrow>vs. size' v)+1" |
 "size' (Clo f vs n) = (size' f + (\<Sum>v\<leftarrow>vs. size' v))+1" |
@@ -581,7 +776,7 @@ apply (simp_all add:map_compose[symmetric])
     apply simp
    apply(erule meta_allE)
    apply(erule meta_mp)
-   apply(simp add:cons_ML_def size'_lift_ML split:nat.split)
+   apply(simp add: size'_lift_ML split:nat.split)
   apply(rule arg_cong[where f = listsum])
   apply(rule map_ext)
   apply simp
@@ -611,14 +806,14 @@ apply simp
 done
 
 function kernel  :: "ml \<Rightarrow> tm"  ("_!" 300) where
-"(C_ML nm)! = C nm" |
-"(A_ML v vs)! = v! \<bullet>\<bullet> (map kernel (rev vs))" |
-"(Lam_ML v)! = \<Lambda> (((lift 0 v)[V\<^isub>U 0 []/0])!)" |
+"(C\<^bsub>ML\<^esub> nm)! = C nm" |
+"(A\<^bsub>ML\<^esub> v vs)! = v! \<bullet>\<bullet> (map kernel (rev vs))" |
+"(Lam\<^bsub>ML\<^esub> v)! = \<Lambda> (((lift 0 v)[V\<^isub>U 0 []/0])!)" |
 "(C\<^isub>U nm vs)! = (C nm) \<bullet>\<bullet> (map kernel (rev vs))" |
 "(V\<^isub>U x vs)! = (V x) \<bullet>\<bullet> (map kernel (rev vs))" |
 "(Clo f vs n)! = f! \<bullet>\<bullet> (map kernel (rev vs))" |
 "(apply v w)! = v! \<bullet> (w!)" |
-"(V_ML X)! = undefined"
+"(V\<^bsub>ML\<^esub> X)! = undefined"
 by pat_completeness auto
 termination by(relation "measure size'") auto
 
@@ -650,19 +845,16 @@ lemma pure_foldl:
 by(induct ts arbitrary: t) simp_all
 
 lemma pure_kernel: fixes v :: ml shows "closed\<^bsub>ML\<^esub> 0 v \<Longrightarrow> pure(v!)"
-apply(induct v rule:kernel.induct)
-apply (auto simp:pure_foldl)
-apply(rule pure.intros)
-apply(erule meta_mp)
-apply(subgoal_tac "closed\<^bsub>ML\<^esub> (Suc 0) (lift 0 v)")
-apply(subgoal_tac "closed\<^bsub>ML\<^esub> 0 (subst\<^bsub>ML\<^esub> (\<lambda>n. V\<^isub>U 0 []) (lift 0 v))")
-apply(drule subst_ML_coincidence[of _ _ "\<lambda>n. V\<^isub>U 0 []" "\<lambda>n. if n = 0 then V\<^isub>U 0 [] else V_ML (n - 1)"])back
-apply simp
-apply metis
-apply simp
-apply(rule closed_ML_subst_ML)
-apply simp+
-done
+proof(induct v rule:kernel.induct)
+  case (3 v)
+  hence "closed\<^bsub>ML\<^esub> (Suc 0) (lift 0 v)" by simp
+  then have "subst\<^bsub>ML\<^esub> (\<lambda>n. V\<^isub>U 0 []) (lift 0 v) = lift 0 v[V\<^isub>U 0 []/0]"
+    by(rule subst_ML_coincidence) simp
+  moreover have "closed\<^bsub>ML\<^esub> 0 (subst\<^bsub>ML\<^esub> (\<lambda>n. V\<^isub>U 0 []) (lift 0 v))"
+    by(simp add: closed_ML_subst_ML)
+  ultimately have "closed\<^bsub>ML\<^esub> 0 (lift 0 v[V\<^isub>U 0 []/0])" by simp
+  thus ?case using 3(1) by (simp add:pure_foldl)
+qed (simp_all add:pure_foldl)
 
 corollary subst_V_kernel: fixes v :: ml shows
   "closed\<^bsub>ML\<^esub> 0 v \<Longrightarrow> subst V (v!) = v!"
@@ -681,7 +873,7 @@ apply(erule_tac x="Suc i" in meta_allE)
 apply(erule meta_impE)
 defer
 apply (simp add:lift_subst_ML)
-apply(subgoal_tac "lift (Suc i) \<circ> (\<lambda>n. if n = 0 then V\<^isub>U 0 [] else V_ML (n - 1)) = (\<lambda>n. if n = 0 then V\<^isub>U 0 [] else V_ML (n - 1))")
+apply(subgoal_tac "lift (Suc i) \<circ> (\<lambda>n. if n = 0 then V\<^isub>U 0 [] else V\<^bsub>ML\<^esub> (n - 1)) = (\<lambda>n. if n = 0 then V\<^isub>U 0 [] else V\<^bsub>ML\<^esub> (n - 1))")
 apply (simp add:lift_lift_ml)
 apply(rule ext)
 apply(simp)
@@ -697,10 +889,10 @@ text{* This function is only introduced to prove the involved susbtitution
 lemma @{text kernel_subst1} below. *}
 
 fun subst_ml :: "(nat \<Rightarrow> nat) \<Rightarrow> ml \<Rightarrow> ml" where
-"subst_ml \<sigma> (C_ML nm) = C_ML nm" |
-"subst_ml \<sigma> (V_ML X) = V_ML X" |
-"subst_ml \<sigma> (A_ML v vs) = A_ML (subst_ml \<sigma> v) (map (subst_ml \<sigma>) vs)" |
-"subst_ml \<sigma> (Lam_ML v) = Lam_ML (subst_ml \<sigma> v)" |
+"subst_ml \<sigma> (C\<^bsub>ML\<^esub> nm) = C\<^bsub>ML\<^esub> nm" |
+"subst_ml \<sigma> (V\<^bsub>ML\<^esub> X) = V\<^bsub>ML\<^esub> X" |
+"subst_ml \<sigma> (A\<^bsub>ML\<^esub> v vs) = A\<^bsub>ML\<^esub> (subst_ml \<sigma> v) (map (subst_ml \<sigma>) vs)" |
+"subst_ml \<sigma> (Lam\<^bsub>ML\<^esub> v) = Lam\<^bsub>ML\<^esub> (subst_ml \<sigma> v)" |
 "subst_ml \<sigma> (C\<^isub>U nm vs) = C\<^isub>U nm (map (subst_ml \<sigma>) vs)" |
 "subst_ml \<sigma> (V\<^isub>U x vs) = V\<^isub>U (\<sigma> x) (map (subst_ml \<sigma>) vs)" |
 "subst_ml \<sigma> (Clo v vs n) = Clo (subst_ml \<sigma> v) (map (subst_ml \<sigma>) vs) n" |
@@ -716,10 +908,10 @@ lemma subst_ml_subst_ML:
   "subst_ml \<sigma> (subst\<^bsub>ML\<^esub> \<sigma>' v) = subst\<^bsub>ML\<^esub> (subst_ml \<sigma> o \<sigma>') (subst_ml \<sigma> v)"
 apply (induct \<sigma>' v arbitrary: \<sigma> rule: subst_ML.induct)
 apply(simp_all add:list_eq_iff_nth_eq)
-apply(subgoal_tac "(subst_ml \<sigma>' \<circ> V_ML 0 ## \<sigma>) = V_ML 0 ## (subst_ml \<sigma>' \<circ> \<sigma>)")
+apply(subgoal_tac "(subst_ml \<sigma>' \<circ> V\<^bsub>ML\<^esub> 0 ## \<sigma>) = V\<^bsub>ML\<^esub> 0 ## (subst_ml \<sigma>' \<circ> \<sigma>)")
 apply simp
 apply(rule ext)
-apply(simp add:cons_ML_def lift_ML_subst_ml split:nat.split)
+apply(simp add: lift_ML_subst_ml)
 done
 
 
@@ -747,18 +939,16 @@ apply simp
 apply(subgoal_tac "(\<lambda>n. V(case n of 0 \<Rightarrow> 0 | Suc k \<Rightarrow> Suc (\<sigma> k))) = (V 0 ## (\<lambda>n. V(\<sigma> n)))")
 apply (simp add:subst_ml_subst_ML)
 defer
-apply(simp add:expand_fun_eq cons_def split:nat.split)
-apply(simp add:cons_def)
-defer
+apply(simp add:expand_fun_eq split:nat.split)
 apply(simp add:lift_is_subst_ml subst_ml_comp)
 apply(rule arg_cong[where f = kernel])
 apply(subgoal_tac "(nat_case 0 (\<lambda>k. Suc (\<sigma> k)) \<circ> Suc) = Suc o \<sigma>")
 prefer 2 apply(simp add:expand_fun_eq split:nat.split)
 apply(subgoal_tac "(subst_ml (nat_case 0 (\<lambda>k. Suc (\<sigma> k))) \<circ>
-               (\<lambda>n. if n = 0 then V\<^isub>U 0 [] else V_ML (n - 1)))
-             = (\<lambda>n. if n = 0 then V\<^isub>U 0 [] else V_ML (n - 1))")
+               (\<lambda>n. if n = 0 then V\<^isub>U 0 [] else V\<^bsub>ML\<^esub> (n - 1)))
+             = (\<lambda>n. if n = 0 then V\<^isub>U 0 [] else V\<^bsub>ML\<^esub> (n - 1))")
 apply simp
-apply(simp add: expand_fun_eq split:nat.split)
+apply(simp add: expand_fun_eq)
 done
 
 lemma if_cong0: "If x y z = If x y z"
@@ -776,7 +966,7 @@ proof(induct u arbitrary:v rule:kernel.induct)
     also have "\<dots> = \<Lambda>((lift 0 w)[lift\<^bsub>ML\<^esub> 0 (lift 0 v)/Suc 0][V\<^isub>U 0 []/0]!)"
       by(simp only: lift_subst_ML1 lift_lift_ML_comm)
     also have "\<dots> = \<Lambda>(subst\<^bsub>ML\<^esub> (\<lambda>n. if n=0 then V\<^isub>U 0 [] else
-            if n=Suc 0 then lift 0 v else V_ML (n - 2)) (lift 0 w) !)"
+            if n=Suc 0 then lift 0 v else V\<^bsub>ML\<^esub> (n - 2)) (lift 0 w) !)"
       apply simp
       apply(rule arg_cong[where f = kernel])
       apply(rule subst_ML_comp2)
@@ -814,7 +1004,7 @@ proof(induct u arbitrary:v rule:kernel.induct)
     finally have "?L = ?M" .
     have "?R = \<Lambda> (subst (V 0 ## subst_decr 0 (v!))
           (lift 0 (lift_ml 0 w[V\<^isub>U 0 []/Suc 0])[V\<^isub>U 0 []/0]!))"
-      apply(subgoal_tac "(V_ML 0 ## (\<lambda>n. if n = 0 then V\<^isub>U 0 [] else V_ML (n - Suc 0))) = subst_decr_ML (Suc 0) (V\<^isub>U 0 [])")
+      apply(subgoal_tac "(V\<^bsub>ML\<^esub> 0 ## (\<lambda>n. if n = 0 then V\<^isub>U 0 [] else V\<^bsub>ML\<^esub> (n - Suc 0))) = subst_decr_ML (Suc 0) (V\<^isub>U 0 [])")
       apply(simp cong:if_cong)
       apply(simp add:expand_fun_eq cons_ML_def split:nat.splits)
       done
@@ -829,7 +1019,7 @@ proof(induct u arbitrary:v rule:kernel.induct)
                (lift 0 (lift_ml 0 w))[V\<^isub>U 0 []/0][V\<^isub>U 1 []/ 0]" (is "?l = ?r")
     proof -
       have "?l = subst\<^bsub>ML\<^esub> (\<lambda>n. if n= 0 then V\<^isub>U 0 [] else if n = 1 then V\<^isub>U 1 [] else
-                      V_ML (n - 2))
+                      V\<^bsub>ML\<^esub> (n - 2))
                (lift_ml 0 (lift_ml 0 w))"
       by(auto intro!:subst_ML_comp2)
     also have "\<dots> = ?r" by(auto intro!:subst_ML_comp2[symmetric])
@@ -919,38 +1109,77 @@ abbreviation "comp_fixed t \<equiv> compile t (\<lambda>i. V\<^isub>U i [])"
 
 text{* Compiled rules: *}
 
+lemma size_args_less_size_tm[simp]: "s \<in> set (args_tm t) \<Longrightarrow> size s < size t"
+by(induct t) auto
+
+fun comp_pat where
+"comp_pat t =
+   (case head_tm t of
+     C nm \<Rightarrow> C\<^isub>U nm (map comp_pat (rev (args_tm t)))
+   | V X \<Rightarrow> V\<^bsub>ML\<^esub> X)"
+
+declare comp_pat.simps[simp del] size_args_less_size_tm[simp del]
+
+lemma comp_pat_V[simp]: "comp_pat(V X) = V\<^bsub>ML\<^esub> X"
+by(simp add:comp_pat.simps)
+
+lemma comp_pat_C[simp]:
+  "comp_pat(C nm \<bullet>\<bullet> ts) = C\<^isub>U nm (map comp_pat (rev ts))"
+by(simp add:comp_pat.simps)
+
+lemma comp_pat_C_Nil[simp]: "comp_pat(C nm) = C\<^isub>U nm []"
+by(simp add:comp_pat.simps)
+
+
 defs compR_def:
- "compR \<equiv> (\<lambda>(nm,ts,t). (nm, map comp_open (rev ts), comp_open t)) ` R \<union>
-     (\<lambda>(nm,ts,t). let vs = map V\<^bsub>ML\<^esub> [0..<arity nm] in (nm, vs, C\<^isub>U nm vs)) ` R"
+ "compR \<equiv> (\<lambda>(nm,ts,t). (nm, map comp_pat (rev ts), comp_open t)) ` R"
 
-text{* Axioms about @{text R}: *}
 
-axiomatization where
-pure_R: "(nm,ts,t) : R \<Longrightarrow> (\<forall>t \<in> set ts. pure t) \<and> pure t"
+lemma fv_ML_comp_open: "pure t \<Longrightarrow> fv\<^bsub>ML\<^esub>(comp_open t) = fv t"
+by(induct t pred:pure) (simp_all add:comp_open_def)
+
+lemma fv_ML_comp_pat: "pattern t \<Longrightarrow> fv\<^bsub>ML\<^esub>(comp_pat t) = fv t"
+by(induct t pred:pattern)(simp_all add:comp_open_def)
+
+lemma fv_compR_aux:
+  "(nm,ts,t') : R \<Longrightarrow> x \<in> fv\<^bsub>ML\<^esub> (comp_open t')
+   \<Longrightarrow> \<exists>t\<in>set ts. x \<in> fv\<^bsub>ML\<^esub>(comp_pat t)"
+apply(frule pure_R)
+apply(simp add:fv_ML_comp_open)
+apply(frule (1) fv_R)
+apply clarsimp
+apply(rule bexI) prefer 2 apply assumption
+apply(drule pattern_R)
+apply(simp add:fv_ML_comp_pat)
+done
+
+lemma fv_compR:
+  "(nm,vs,v) : compR \<Longrightarrow> x \<in> fv\<^bsub>ML\<^esub> v \<Longrightarrow> \<exists>u\<in>set vs. x \<in> fv\<^bsub>ML\<^esub> u"
+by(fastsimp simp add:compR_def image_def dest: fv_compR_aux)
 
 lemma lift_compile:
- "pure t \<Longrightarrow> \<forall>\<sigma> k. lift k (compile t \<sigma>) = compile t (lift k \<circ> \<sigma>)"
+  "pure t \<Longrightarrow> \<forall>\<sigma> k. lift k (compile t \<sigma>) = compile t (lift k \<circ> \<sigma>)"
 apply(induct pred:pure)
 apply simp_all
 apply clarsimp
 apply(rule_tac f = "compile t" in arg_cong)
 apply(rule ext)
-apply (clarsimp simp:cons_ML_def lift_lift_ML_comm split:nat.split)
+apply (clarsimp simp: lift_lift_ML_comm)
 done
 
 lemma subst_ML_compile:
   "pure t \<Longrightarrow> subst\<^bsub>ML\<^esub> \<sigma>' (compile t \<sigma>) = compile t (subst\<^bsub>ML\<^esub> \<sigma>' o \<sigma>)"
 apply(induct arbitrary: \<sigma> \<sigma>' pred:pure)
 apply simp_all
-apply(erule_tac x="V_ML 0 ## \<sigma>'" in meta_allE)
-apply(erule_tac x= "V_ML 0 ## (lift\<^bsub>ML\<^esub> 0 \<circ> \<sigma>)" in meta_allE)
+apply(erule_tac x="V\<^bsub>ML\<^esub> 0 ## \<sigma>'" in meta_allE)
+apply(erule_tac x= "V\<^bsub>ML\<^esub> 0 ## (lift\<^bsub>ML\<^esub> 0 \<circ> \<sigma>)" in meta_allE)
 apply(rule_tac f = "compile t" in arg_cong)
 apply(rule ext)
-apply (auto simp add:subst_ML_ext cons_ML_def lift_ML_subst_ML split:nat.split)
+apply (auto simp add:subst_ML_ext lift_ML_subst_ML)
 done
 
 theorem kernel_compile:
- "pure t \<Longrightarrow> \<forall>i. \<sigma> i = V\<^isub>U i [] \<Longrightarrow> (compile t \<sigma>)! = t"
+  "pure t \<Longrightarrow> \<forall>i. \<sigma> i = V\<^isub>U i [] \<Longrightarrow> (compile t \<sigma>)! = t"
 apply(induct arbitrary: \<sigma> pred:pure)
 apply simp_all
 apply(subst lift_compile) apply simp
@@ -959,7 +1188,19 @@ apply(subgoal_tac "(subst\<^bsub>ML\<^esub> (\<lambda>n. if n = 0 then V\<^isub>
                (lift 0 \<circ> V\<^bsub>ML\<^esub> 0 ## \<sigma>)) = (\<lambda>a. V\<^isub>U a [])")
 apply(simp)
 apply(rule ext)
-apply(simp add:cons_ML_def split:nat.split)
+apply(simp)
+done
+
+lemma kernel_subst_ML_pat:
+  "pure t \<Longrightarrow> pattern t \<Longrightarrow> \<forall>i. closed\<^bsub>ML\<^esub> 0 (\<sigma> i) \<Longrightarrow>
+   (subst\<^bsub>ML\<^esub> \<sigma> (comp_pat t))! = subst (kernel \<circ> \<sigma>) t"
+apply(induct arbitrary: \<sigma> pred:pure)
+apply simp_all
+apply(frule pattern_At_decomp)
+apply(frule pattern_AtD12)
+apply clarsimp
+apply(subst comp_pat.simps)
+apply(simp add: rev_map)
 done
 
 lemma kernel_subst_ML:
@@ -967,65 +1208,67 @@ lemma kernel_subst_ML:
    (subst\<^bsub>ML\<^esub> \<sigma> (comp_open t))! = subst (kernel \<circ> \<sigma>) t"
 proof(induct arbitrary: \<sigma> pred:pure)
   case (Lam t)
-  have "lift 0 o V_ML = V_ML" by (simp add:expand_fun_eq)
+  have "lift 0 o V\<^bsub>ML\<^esub> = V\<^bsub>ML\<^esub>" by (simp add:expand_fun_eq)
   hence "(subst\<^bsub>ML\<^esub> \<sigma> (comp_open (\<Lambda> t)))! =
     \<Lambda> (subst\<^bsub>ML\<^esub> (lift 0 \<circ> V\<^bsub>ML\<^esub> 0 ## \<sigma>) (comp_open t)[V\<^isub>U 0 []/0]!)"
     using Lam by(simp add: lift_subst_ML comp_open_def lift_compile)
   also have "\<dots> = \<Lambda> (subst (V 0 ## (kernel \<circ> \<sigma>)) t)" using Lam
-    by(simp add: subst_ML_comp subst_ext cons_ML_def cons_def kernel_lift_tm
-      split:nat.split)
+    by(simp add: subst_ML_comp subst_ext kernel_lift_tm)
   also have "\<dots> = subst (kernel o \<sigma>) (\<Lambda> t)" by simp
   finally show ?case .
 qed (simp_all add:comp_open_def)
 
-lemma kernel_subst_ML_map:
-  "\<forall>t \<in> set ts. pure t \<Longrightarrow> \<forall>i. closed\<^bsub>ML\<^esub> 0 (\<sigma> i) \<Longrightarrow>
-   map kernel (map (subst\<^bsub>ML\<^esub> \<sigma>) (map comp_open ts)) =
+lemma kernel_subst_ML_pat_map:
+  "\<forall>t \<in> set ts. pure t \<and> pattern t \<Longrightarrow> \<forall>i. closed\<^bsub>ML\<^esub> 0 (\<sigma> i) \<Longrightarrow>
+   map kernel (map (subst\<^bsub>ML\<^esub> \<sigma>) (map comp_pat ts)) =
    map (subst (kernel \<circ> \<sigma>)) ts"
-by(simp add:list_eq_iff_nth_eq kernel_subst_ML)
+by(simp add:list_eq_iff_nth_eq kernel_subst_ML_pat)
 
-lemma compR_tRed: "(nm, vs, v) : compR \<Longrightarrow> \<forall> i. closed\<^bsub>ML\<^esub> 0 (\<sigma> i)
+lemma compR_Red_tm: "(nm, vs, v) : compR \<Longrightarrow> \<forall> i. closed\<^bsub>ML\<^esub> 0 (\<sigma> i)
   \<Longrightarrow> C nm \<bullet>\<bullet> (map (subst\<^bsub>ML\<^esub> \<sigma>) (rev vs))! \<rightarrow>* (subst\<^bsub>ML\<^esub> \<sigma> v)!"
 apply(auto simp add:compR_def rev_map)
 apply(frule pure_R)
 apply(subst kernel_subst_ML) apply fast+
-apply(subst kernel_subst_ML_map) apply fast+
+apply(subst kernel_subst_ML_pat_map)
+ apply(fast dest:pattern_R)
+ apply assumption
 apply(rule r_into_rtrancl)
-apply(erule tRed.intros)
+apply(erule Red_tm.intros)
 done
+
 
 section "Correctness"
 
 (* Without this special rule one "also" in the next proof *diverges*,
    probably because of HOU. *)
-lemma eq_tRed_trans: "s = t \<Longrightarrow> t \<rightarrow> t' \<Longrightarrow> s \<rightarrow> t'"
+lemma eq_Red_tm_trans: "s = t \<Longrightarrow> t \<rightarrow> t' \<Longrightarrow> s \<rightarrow> t'"
 by simp
 
 text{* Soundness of reduction: *}
-theorem fixes v :: ml shows Red_sound:
+theorem fixes v :: ml shows Red_ml_sound:
   "v \<Rightarrow> v' \<Longrightarrow> closed\<^bsub>ML\<^esub> 0 v \<Longrightarrow> v! \<rightarrow>* v'! \<and> closed\<^bsub>ML\<^esub> 0 v'" and
   "vs \<Rightarrow> vs' \<Longrightarrow> \<forall>v\<in>set vs. closed\<^bsub>ML\<^esub> 0 v \<Longrightarrow>
    vs! \<rightarrow>* vs'! \<and> (\<forall>v'\<in>set vs'. closed\<^bsub>ML\<^esub> 0 v')"
-proof(induct rule:Red_Redl.inducts)
+proof(induct rule:Red_ml_Red_ml_list.inducts)
   fix u v
-  let ?v = "A_ML (Lam_ML u) [v]"
-  assume cl: "closed\<^bsub>ML\<^esub> 0 (A_ML (Lam_ML u) [v])"
+  let ?v = "A\<^bsub>ML\<^esub> (Lam\<^bsub>ML\<^esub> u) [v]"
+  assume cl: "closed\<^bsub>ML\<^esub> 0 (A\<^bsub>ML\<^esub> (Lam\<^bsub>ML\<^esub> u) [v])"
   let ?u' = "(lift_ml 0 u)[V\<^isub>U 0 []/0]"
   have "?v! = (\<Lambda>((?u')!)) \<bullet> (v !)" by simp
-  also have "\<dots> \<rightarrow> (?u' !)[v!/0]" (is "_ \<rightarrow> ?R") by(rule tRed.intros)
-  also(eq_tRed_trans) have "?R = u[v/0]!" using cl
+  also have "\<dots> \<rightarrow> (?u' !)[v!/0]" (is "_ \<rightarrow> ?R") by(rule Red_tm.intros)
+  also(eq_Red_tm_trans) have "?R = u[v/0]!" using cl
     apply(cut_tac u = "u" and v = "v" in kernel_subst1)
     apply(simp_all)
     done
-  finally have "kernel(A_ML (Lam_ML u) [v]) \<rightarrow>* kernel(u[v/0])" (is ?A)
+  finally have "kernel(A\<^bsub>ML\<^esub> (Lam\<^bsub>ML\<^esub> u) [v]) \<rightarrow>* kernel(u[v/0])" (is ?A)
     by(rule r_into_rtrancl)
   moreover have "closed\<^bsub>ML\<^esub> 0 (u[v/0])" (is "?C")
   proof -
-    let ?\<sigma> = "\<lambda>n. if n = 0 then v else V_ML (n - 1)"
+    let ?\<sigma> = "\<lambda>n. if n = 0 then v else V\<^bsub>ML\<^esub> (n - 1)"
     let ?\<sigma>' = "\<lambda>n. v"
     have clu: "closed\<^bsub>ML\<^esub> (Suc 0) u" and clv: "closed\<^bsub>ML\<^esub> 0 v" using cl by simp+
     have "closed\<^bsub>ML\<^esub> 0 (subst\<^bsub>ML\<^esub> ?\<sigma>' u)"
-      by (metis COMBK_def closed_ML_subst_ML clv)
+      by (metis closed_ML_subst_ML clv)
     hence "closed\<^bsub>ML\<^esub> 0 (subst\<^bsub>ML\<^esub> ?\<sigma> u)"
       using subst_ML_coincidence[OF clu, of ?\<sigma> ?\<sigma>'] by auto
     thus ?thesis by simp
@@ -1036,19 +1279,19 @@ next
   assume \<sigma>: "\<forall>i. closed\<^bsub>ML\<^esub> 0 (\<sigma> i)"  and compR: "(nm, vs, v) \<in> compR"
   have "map (subst V) (map (subst\<^bsub>ML\<^esub> \<sigma>) (rev vs)!) = map (subst\<^bsub>ML\<^esub> \<sigma>) (rev vs)!"
     by(simp add:list_eq_iff_nth_eq subst_V_kernel closed_ML_subst_ML[OF \<sigma>])
-  with compR_tRed[OF compR \<sigma>]
+  with compR_Red_tm[OF compR \<sigma>]
   have "(C nm) \<bullet>\<bullet> ((map (subst\<^bsub>ML\<^esub> \<sigma>) (rev vs)) !) \<rightarrow>* (subst\<^bsub>ML\<^esub> \<sigma> v)!"
     by(simp add:subst_V_kernel closed_ML_subst_ML[OF \<sigma>])
-  hence "A_ML (C_ML nm) (map (subst\<^bsub>ML\<^esub> \<sigma>) vs)! \<rightarrow>* subst\<^bsub>ML\<^esub> \<sigma> v!" (is ?A)
+  hence "A\<^bsub>ML\<^esub> (C\<^bsub>ML\<^esub> nm) (map (subst\<^bsub>ML\<^esub> \<sigma>) vs)! \<rightarrow>* subst\<^bsub>ML\<^esub> \<sigma> v!" (is ?A)
     by(simp add:rev_map)
   moreover
   have "closed\<^bsub>ML\<^esub> 0 (subst\<^bsub>ML\<^esub> \<sigma> v)" (is ?C) by(metis closed_ML_subst_ML \<sigma>)
   ultimately show "?A \<and> ?C" ..
-qed (auto simp:tRed_list_foldl_At tRed_rev rev_map[symmetric])
+qed (auto simp:Reds_tm_list_foldl_At Red_tm_rev rev_map[symmetric])
 
-theorem Redt_sound:
+theorem Red_term_sound:
   "t \<Rightarrow> t' \<Longrightarrow> closed\<^bsub>ML\<^esub> 0 t \<Longrightarrow> kernelt t \<rightarrow>* kernelt t'  \<and> closed\<^bsub>ML\<^esub> 0 t'"
-proof(induct rule:Redt.inducts)
+proof(induct rule:Red_term.inducts)
   case term_C thus ?case
     by (auto simp:closed_tm_ML_foldl_At map_compose[symmetric])
 next
@@ -1064,44 +1307,1042 @@ next
   hence "term (Clo vf vs n)! \<rightarrow>*
        \<Lambda> (term (apply (lift 0 (Clo vf vs n)) (V\<^isub>U 0 [])))!"
     using term_Clo
-    by(simp del:lift_foldl_At add: r_into_rtrancl tRed.intros(2))
+    by(simp del:lift_foldl_At add: r_into_rtrancl Red_tm.intros(2))
   moreover
   have "closed\<^bsub>ML\<^esub> 0 (\<Lambda> (term (apply (lift 0 (Clo vf vs n)) (V\<^isub>U 0 []))))"
     using term_Clo by simp
   ultimately show ?case ..
 next
-  case ctxt_term thus ?case by simp (metis Red_sound)
+  case ctxt_term thus ?case by simp (metis Red_ml_sound)
 qed auto
 
 corollary kernel_inv:
  "(t :: tm) \<Rightarrow>* t' \<Longrightarrow> closed\<^bsub>ML\<^esub> 0 t \<Longrightarrow> t! \<rightarrow>* t'! \<and> closed\<^bsub>ML\<^esub> 0 t' "
 apply(induct rule: rtrancl.induct)
 apply (metis rtrancl_eq_or_trancl)
-apply (metis Redt_sound rtrancl_trans)
+apply (metis Red_term_sound rtrancl_trans)
 done
 
 lemma  closed_ML_compile:
   "pure t \<Longrightarrow> \<forall>i. closed\<^bsub>ML\<^esub> n (\<sigma> i) \<Longrightarrow> closed\<^bsub>ML\<^esub> n (compile t \<sigma>)"
 proof(induct arbitrary:n \<sigma> pred:pure)
   case (Lam t)
-  have 1: "\<forall>i. closed\<^bsub>ML\<^esub> (Suc n) ((V_ML 0 ## \<sigma>) i)" using Lam(3-)
-    by (auto simp: closed_ML_Suc cons_ML_def split:nat.split)
-    show ?case using Lam(2)[OF 1] by simp
+  have 1: "\<forall>i. closed\<^bsub>ML\<^esub> (Suc n) ((V\<^bsub>ML\<^esub> 0 ## \<sigma>) i)" using Lam(3-)
+    by (auto simp: closed_ML_Suc)
+  show ?case using Lam(2)[OF 1] by (simp del:apply_cons_ML)
 qed simp_all
 
 theorem nbe_correct: fixes t :: tm
-assumes "pure t" and "pure t'"
-and "term (comp_fixed t) \<Rightarrow>* t'" shows "t \<rightarrow>* t'"
+assumes "pure t" and "term (comp_fixed t) \<Rightarrow>* t'" and "pure t'" shows "t \<rightarrow>* t'"
 proof -
   have ML_cl: "closed\<^bsub>ML\<^esub> 0 (term (comp_fixed t))"
     by (simp add: closed_ML_compile[OF `pure t`])
   have "(term (comp_fixed t))! = t"
     using kernel_compile[OF `pure t`] by simp
   moreover have "term (comp_fixed t)! \<rightarrow>* t'!"
-    using kernel_inv[OF assms(3) ML_cl] by auto
+    using kernel_inv[OF assms(2) ML_cl] by auto
   ultimately have "t \<rightarrow>* t'!" by simp
   thus ?thesis using kernel_pure[OF `pure t'`] by simp
 qed
+
+
+section "Normal Forms"
+
+inductive normal :: "tm \<Rightarrow> bool" where
+"\<forall>t\<in>set ts. normal t \<Longrightarrow> normal(V x \<bullet>\<bullet> ts)" |
+"normal t \<Longrightarrow> normal(\<Lambda> t)" |
+"\<forall>t\<in>set ts. normal t \<Longrightarrow>
+ \<forall>\<sigma>. \<forall>(nm',ls,r)\<in>R. \<not>(nm = nm' \<and> take (size ls) ts = map (subst \<sigma>) ls)
+ \<Longrightarrow> normal(C nm \<bullet>\<bullet> ts)"
+
+fun C_normal_ML :: "ml \<Rightarrow> bool" ("C'_normal\<^bsub>ML\<^esub>") where
+"C_normal\<^bsub>ML\<^esub>(C\<^isub>U nm vs) =
+  ((\<forall>v\<in>set vs. C_normal\<^bsub>ML\<^esub> v) \<and> no_match_compR nm vs)" |
+"C_normal\<^bsub>ML\<^esub> (C\<^bsub>ML\<^esub> _) = True" |
+"C_normal\<^bsub>ML\<^esub> (V\<^bsub>ML\<^esub> _) = True" |
+"C_normal\<^bsub>ML\<^esub> (A\<^bsub>ML\<^esub> v vs) = (C_normal\<^bsub>ML\<^esub> v \<and> (\<forall>v \<in> set vs. C_normal\<^bsub>ML\<^esub> v))" |
+"C_normal\<^bsub>ML\<^esub> (Lam\<^bsub>ML\<^esub> v) = C_normal\<^bsub>ML\<^esub> v" |
+"C_normal\<^bsub>ML\<^esub> (V\<^isub>U x vs) = (\<forall>v \<in> set vs. C_normal\<^bsub>ML\<^esub> v)" |
+"C_normal\<^bsub>ML\<^esub> (Clo v vs _) = (C_normal\<^bsub>ML\<^esub> v \<and> (\<forall>v \<in> set vs. C_normal\<^bsub>ML\<^esub> v))" |
+"C_normal\<^bsub>ML\<^esub> (apply u v) = (C_normal\<^bsub>ML\<^esub> u \<and> C_normal\<^bsub>ML\<^esub> v)"
+
+fun size_tm :: "tm \<Rightarrow> nat" where
+"size_tm (C _) = 1" |
+"size_tm (At s t) = size_tm s + size_tm t + 1" |
+"size_tm _ = 0"
+
+lemma size_tm_foldl_At: "size_tm(t \<bullet>\<bullet> ts) = size_tm t + list_size size_tm ts"
+by (induct ts arbitrary:t) auto
+
+lemma termination_no_match:
+  "i < length ss \<Longrightarrow> ss ! i = C nm \<bullet>\<bullet> ts
+   \<Longrightarrow> listsum (map size_tm ts) < listsum (map size_tm ss)"
+apply(subgoal_tac "C nm \<bullet>\<bullet> ts : set ss")
+ apply(drule listsum_map_remove1[of _ _ size_tm])
+apply(simp add:size_tm_foldl_At list_size_conv_listsum)
+apply (metis in_set_conv_nth)
+done
+
+declare conj_cong [fundef_cong]
+
+function no_match :: "tm list \<Rightarrow> tm list \<Rightarrow> bool" where
+"no_match ps ts =
+  (\<exists>i < min (size ts) (size ps).
+   \<exists>nm nm' rs rs'. ps!i = (C nm) \<bullet>\<bullet> rs \<and> ts!i = (C nm') \<bullet>\<bullet> rs' \<and>
+      (nm=nm' \<longrightarrow> no_match rs rs'))"
+by pat_completeness auto
+termination
+apply(relation "measure(%(ts::tm list,_). \<Sum>t\<leftarrow>ts. size_tm t)")
+apply (auto simp:termination_no_match)
+done
+
+declare no_match.simps[simp del]
+
+abbreviation
+"no_match_R nm ts \<equiv> \<forall>(nm',ps,t)\<in> R. nm=nm' \<longrightarrow> no_match ps ts"
+
+
+lemma no_match: "no_match ps ts \<Longrightarrow> \<not>(\<exists>\<sigma>. map (subst \<sigma>) ps = ts)"
+proof(induct ps ts rule:no_match.induct)
+  case (1 ps ts)
+  thus ?case
+    apply auto
+    apply(subst (asm) no_match.simps[of ps])
+    apply fastsimp
+    done
+qed
+
+lemma no_match_take: "no_match ps ts \<Longrightarrow> no_match ps (take (size ps) ts)"
+apply(subst (asm) no_match.simps)
+apply(subst no_match.simps)
+apply fastsimp
+done
+
+fun dterm_ML :: "ml \<Rightarrow> tm" ("dterm\<^bsub>ML\<^esub>") where
+"dterm\<^bsub>ML\<^esub> (C\<^isub>U nm vs) = C nm \<bullet>\<bullet> map dterm\<^bsub>ML\<^esub> (rev vs)" |
+"dterm\<^bsub>ML\<^esub> _ = V 0"
+
+fun dterm :: "tm \<Rightarrow> tm" where
+"dterm (V n) = V n" |
+"dterm (C nm) = C nm" |
+"dterm (s \<bullet> t) = dterm s \<bullet> dterm t" |
+"dterm (\<Lambda> t) = \<Lambda> (dterm t)" |
+"dterm (term v) = dterm\<^bsub>ML\<^esub> v"
+
+lemma dterm_pure[simp]: "pure t \<Longrightarrow> dterm t = t"
+by (induct pred:pure) auto
+
+lemma map_dterm_pure[simp]: "\<forall>t\<in>set ts. pure t \<Longrightarrow> map dterm ts = ts"
+by (induct ts) auto
+
+lemma map_dterm_term[simp]: "map dterm (map term vs) = map dterm\<^bsub>ML\<^esub> vs"
+by (induct vs) auto
+
+lemma dterm_foldl_At[simp]: "dterm(t \<bullet>\<bullet> ts) = dterm t \<bullet>\<bullet> map dterm ts"
+by(induct ts arbitrary: t) auto
+
+lemma no_match_coincide:
+  "no_match\<^bsub>ML\<^esub> ps vs \<Longrightarrow>
+  no_match (map dterm\<^bsub>ML\<^esub> (rev ps)) (map dterm\<^bsub>ML\<^esub> (rev vs))"
+apply(induct ps vs rule:no_match_ML.induct)
+apply(rotate_tac 1)
+apply(subst (asm) no_match_ML.simps)
+apply (elim exE conjE)
+apply(case_tac "nm=nm'")
+prefer 2
+apply(subst no_match.simps)
+apply(rule_tac x=i in exI)
+apply rule
+apply (simp (no_asm))
+apply (metis min_less_iff_conj)
+apply(simp add:min_less_iff_conj nth_map)
+apply safe
+apply(erule_tac x=i in meta_allE)
+apply(erule_tac x=nm' in meta_allE)
+apply(erule_tac x=nm' in meta_allE)
+apply(erule_tac x="vs" in meta_allE)
+apply(erule_tac x="vs'" in meta_allE)
+apply(subst no_match.simps)
+apply(rule_tac x=i in exI)
+apply rule
+apply (simp (no_asm))
+apply (metis min_less_iff_conj)
+apply(rule_tac x=nm' in exI)
+apply(rule_tac x=nm' in exI)
+apply(rule_tac x="map dterm\<^bsub>ML\<^esub> (rev vs)" in exI)
+apply(rule_tac x="map dterm\<^bsub>ML\<^esub> (rev vs')" in exI)
+apply(simp)
+done
+
+lemma dterm_ML_comp_patD:
+  "pattern t \<Longrightarrow> dterm\<^bsub>ML\<^esub> (comp_pat t) = C nm \<bullet>\<bullet> rs \<Longrightarrow> \<exists>ts. t = C nm \<bullet>\<bullet> ts"
+by(induct pred:pattern) simp_all
+
+lemma no_match_R_coincide_aux[rule_format]: "\<forall>t\<in>set ts. pattern t \<Longrightarrow>
+  no_match (map (dterm\<^bsub>ML\<^esub> \<circ> comp_pat) ts) rs \<longrightarrow> no_match ts rs"
+apply(induct ts rs rule:no_match.induct)
+apply(subst (1 2) no_match.simps)
+apply clarsimp
+apply(rule_tac x=i in exI)
+apply simp
+apply(rule_tac x=nm in exI)
+apply(cut_tac t = "ps!i" in dterm_ML_comp_patD, simp, assumption)
+apply(clarsimp)
+apply(erule_tac x = i in meta_allE)
+apply(erule_tac x = nm' in meta_allE)
+apply(erule_tac x = nm' in meta_allE)
+apply(erule_tac x = tsa in meta_allE)
+apply(erule_tac x = rs' in meta_allE)
+apply (simp add:rev_map map_compose[symmetric])
+apply (metis in_set_conv_nth pattern_At_vecD)
+done
+
+lemma no_match_R_coincide:
+  "no_match_compR nm (rev vs) \<Longrightarrow> no_match_R nm (map dterm\<^bsub>ML\<^esub> vs)"
+apply auto
+apply(drule_tac x="(nm, map comp_pat (rev aa), comp_open b)" in bspec)
+ unfolding compR_def
+ apply (simp add:image_def) 
+ apply (force)
+apply (simp)
+apply(drule no_match_coincide)
+apply(frule pure_R)
+apply(drule pattern_R)
+apply(clarsimp simp add: rev_map no_match.simps[of _ "map dterm\<^bsub>ML\<^esub> vs"])
+apply(rule_tac x=i in exI)
+apply simp
+apply(cut_tac t = "aa!i" in dterm_ML_comp_patD, simp, assumption)
+apply clarsimp
+apply(auto simp: rev_map map_compose[symmetric])
+apply(rule no_match_R_coincide_aux)
+prefer 2 apply assumption
+apply (metis in_set_conv_nth pattern_At_vecD)
+done
+
+
+inductive C_normal :: "tm \<Rightarrow> bool" where
+"\<forall>t\<in>set ts. C_normal t \<Longrightarrow> C_normal(V x \<bullet>\<bullet> ts)" |
+"C_normal t \<Longrightarrow> C_normal(\<Lambda> t)" |
+"C_normal\<^bsub>ML\<^esub> v \<Longrightarrow> C_normal(term v)" |
+"\<forall>t\<in>set ts. C_normal t \<Longrightarrow> no_match_R nm (map dterm ts)
+ \<Longrightarrow> C_normal(C nm \<bullet>\<bullet> ts)"
+
+declare C_normal.intros[simp]
+
+lemma C_normal_term[simp]: "C_normal(term v) = C_normal\<^bsub>ML\<^esub> v"
+apply (auto)
+apply(erule C_normal.cases)
+apply auto
+done
+
+lemma [simp]: "C_normal(\<Lambda> t) = C_normal t"
+apply (auto)
+apply(erule C_normal.cases)
+apply auto
+done
+
+lemma [simp]: "C_normal(V x)"
+using C_normal.intros(1)[of "[]" x]
+by simp
+
+lemma [simp]: "dterm (dterm\<^bsub>ML\<^esub> v) = dterm\<^bsub>ML\<^esub> v"
+apply(induct v rule:dterm_ML.induct)
+apply (simp_all add: map_compose[symmetric])
+done
+
+lemma "u\<Rightarrow>(v::ml) \<Longrightarrow> True" and
+  Red_ml_list_length: "vs \<Rightarrow> vs' \<Longrightarrow> length vs = length vs'"
+by(induct rule: Red_ml_Red_ml_list.inducts) simp_all
+
+lemma "(v::ml) \<Rightarrow> v' \<Longrightarrow> True" and
+  Red_ml_list_nth: "(vs::ml list) \<Rightarrow> vs'
+  \<Longrightarrow> \<exists>v' k. k<size vs \<and> vs!k \<Rightarrow> v' \<and> vs' = vs[k := v']"
+apply (induct rule: Red_ml_Red_ml_list.inducts)
+apply (auto split:nat.splits)
+done
+
+lemma Red_ml_list_pres_no_match:
+  "no_match\<^bsub>ML\<^esub> ps vs \<Longrightarrow> vs \<Rightarrow> vs' \<Longrightarrow> no_match\<^bsub>ML\<^esub> ps vs'"
+proof(induct ps vs arbitrary: vs' rule:no_match_ML.induct)
+  case (1 vs os)
+  show ?case using 1(2-3)
+apply-
+apply(frule Red_ml_list_length)
+apply(rotate_tac -2)
+apply(subst (asm) no_match_ML.simps)
+apply clarify
+apply(rename_tac i nm nm' us us')
+apply(subst no_match_ML.simps)
+apply(rule_tac x=i in exI)
+apply (simp)
+apply(drule Red_ml_list_nth)
+apply clarify
+apply(rename_tac k)
+apply(case_tac "k = length os - Suc i")
+prefer 2
+apply(rule_tac x=nm' in exI)
+apply(rule_tac x=us' in exI)
+apply (simp add: rev_nth nth_list_update)
+apply (simp add: rev_nth)
+apply(erule Red_ml.cases)
+apply simp_all
+apply(fastsimp intro: 1(1) simp add:rev_nth)
+done
+qed
+
+lemma no_match_ML_subst_ML[rule_format]:
+  "\<forall>v\<in>set vs. \<forall>x\<in>fv\<^bsub>ML\<^esub> v. C_normal\<^bsub>ML\<^esub> (\<sigma> x) \<Longrightarrow>
+   no_match\<^bsub>ML\<^esub> ps vs \<longrightarrow> no_match\<^bsub>ML\<^esub> ps (map (subst\<^bsub>ML\<^esub> \<sigma>) vs)"
+apply(induct ps vs rule:no_match_ML.induct)
+apply simp
+apply(subst (1 2) no_match_ML.simps)
+apply clarsimp
+apply(rule_tac x=i in exI)
+apply simp
+apply(rule_tac x=nm' in exI)
+apply(rule_tac x="map (subst\<^bsub>ML\<^esub> \<sigma>) vs'" in exI)
+apply (auto simp:rev_nth)
+apply(erule_tac x = i in meta_allE)
+apply(erule_tac x = nm' in meta_allE)
+apply(erule_tac x = nm' in meta_allE)
+apply(erule_tac x = vs in meta_allE)
+apply(erule_tac x = vs' in meta_allE)
+apply simp
+apply (metis UN_I fv_ML.simps(5) in_set_conv_nth length_rev rev_nth set_rev)
+done
+
+lemma lift_is_CUD:
+  "lift\<^bsub>ML\<^esub> k v = C\<^isub>U nm vs' \<Longrightarrow> \<exists>vs. v = C\<^isub>U nm vs \<and> vs' = map (lift\<^bsub>ML\<^esub> k) vs"
+by(cases v) auto
+
+lemma no_match_ML_lift_ML:
+  "no_match\<^bsub>ML\<^esub> ps (map (lift\<^bsub>ML\<^esub> k) vs) = no_match\<^bsub>ML\<^esub> ps vs"
+apply(induct ps vs rule:no_match_ML.induct)
+apply simp
+apply(subst (1 2) no_match_ML.simps)
+apply rule
+ apply clarsimp
+ apply(rule_tac x=i in exI)
+ apply (simp add:rev_nth)
+ apply(drule lift_is_CUD)
+ apply fastsimp
+apply clarsimp
+apply(rule_tac x=i in exI)
+apply simp
+apply(rule_tac x=nm' in exI)
+apply(rule_tac x="map (lift\<^bsub>ML\<^esub> k) vs'" in exI)
+apply (fastsimp simp:rev_nth)
+done
+
+lemma C_normal_ML_lift_ML: "C_normal\<^bsub>ML\<^esub>(lift\<^bsub>ML\<^esub> k v) = C_normal\<^bsub>ML\<^esub> v"
+by(induct v arbitrary: k rule:C_normal_ML.induct)(auto simp:no_match_ML_lift_ML)
+
+lemma no_match_compR_Cons:
+  "no_match_compR nm vs \<Longrightarrow> no_match_compR nm (v # vs)"
+apply auto
+apply(drule bspec, assumption)
+apply simp
+apply(subst (asm) no_match_ML.simps)
+apply(subst no_match_ML.simps)
+apply clarsimp
+apply(rule_tac x=i in exI)
+apply (simp add:nth_append)
+done
+
+lemma C_normal_ML_comp_open: "pure t \<Longrightarrow> C_normal\<^bsub>ML\<^esub>(comp_open t)"
+by (induct pred:pure) (auto simp:comp_open_def)
+
+lemma C_normal_compR_rhs: "(nm, vs, v) \<in> compR \<Longrightarrow> C_normal\<^bsub>ML\<^esub> v"
+by(auto simp: compR_def image_def Bex_def pure_R C_normal_ML_comp_open)
+
+
+lemma C_normal_ML_subst_ML:
+  "C_normal\<^bsub>ML\<^esub> (subst\<^bsub>ML\<^esub> \<sigma> v) \<Longrightarrow> (\<forall>x\<in>fv\<^bsub>ML\<^esub> v. C_normal\<^bsub>ML\<^esub> (\<sigma> x))"
+proof(induct \<sigma> v rule:subst_ML.induct)
+  case 4 thus ?case
+    by(simp del:apply_cons_ML)(force simp add: C_normal_ML_lift_ML)
+      (* weird - force suffices in apply style *)
+qed auto
+
+lemma C_normal_ML_subst_ML_iff: "C_normal\<^bsub>ML\<^esub> v \<Longrightarrow>
+  C_normal\<^bsub>ML\<^esub> (subst\<^bsub>ML\<^esub> \<sigma> v) \<longleftrightarrow> (\<forall>x\<in>fv\<^bsub>ML\<^esub> v. C_normal\<^bsub>ML\<^esub> (\<sigma> x))"
+proof(induct \<sigma> v rule:subst_ML.induct)
+  case 4 thus ?case
+    by(simp del:apply_cons_ML)(force simp add: C_normal_ML_lift_ML)
+      (* weird - force suffices in apply style *)
+next
+  case 5 thus ?case by simp (blast intro: no_match_ML_subst_ML)
+qed auto
+
+lemma C_normal_ML_inv: "v \<Rightarrow> v' \<Longrightarrow> C_normal\<^bsub>ML\<^esub> v \<Longrightarrow> C_normal\<^bsub>ML\<^esub> v'" and
+      "vs \<Rightarrow> vs' \<Longrightarrow> \<forall>v\<in>set vs. C_normal\<^bsub>ML\<^esub> v \<Longrightarrow> \<forall>v'\<in>set vs'. C_normal\<^bsub>ML\<^esub> v'"
+apply(induct rule:Red_ml_Red_ml_list.inducts)
+apply(simp_all add: C_normal_ML_subst_ML_iff)
+  apply(metis C_normal_ML_subst_ML C_normal_compR_rhs
+        fv_compR C_normal_ML_subst_ML_iff)
+ apply(blast intro!:no_match_compR_Cons)
+apply(blast dest:Red_ml_list_pres_no_match)
+done
+
+
+lemma Red_term_hnf_induct[consumes 1]:
+assumes "(t::tm) \<Rightarrow> t'"
+  "\<And>nm vs ts. P ((term (C\<^isub>U nm vs)) \<bullet>\<bullet> ts) ((C nm \<bullet>\<bullet> map term (rev vs)) \<bullet>\<bullet> ts)"
+  "\<And>x vs ts. P (term (V\<^isub>U x vs) \<bullet>\<bullet> ts) ((V x \<bullet>\<bullet> map term (rev vs)) \<bullet>\<bullet> ts)"
+  "\<And>vf vs n ts.
+    P (term (Clo vf vs n) \<bullet>\<bullet> ts)
+     ((\<Lambda> (term (apply (lift 0 (Clo vf vs n)) (V\<^isub>U 0 [])))) \<bullet>\<bullet> ts)"
+  "\<And>t t' ts. \<lbrakk>t \<Rightarrow> t'; P t t'\<rbrakk> \<Longrightarrow> P (\<Lambda> t \<bullet>\<bullet> ts) (\<Lambda> t' \<bullet>\<bullet> ts)"
+  "\<And>v v' ts. v \<Rightarrow> v' \<Longrightarrow> P (term v \<bullet>\<bullet> ts) (term v' \<bullet>\<bullet> ts)"
+  "\<And>x i t' ts. i<size ts \<Longrightarrow> ts!i \<Rightarrow> t' \<Longrightarrow> P (ts!i) (t')
+    \<Longrightarrow> P (V x  \<bullet>\<bullet> ts) (V x \<bullet>\<bullet> ts[i:=t'])"
+  "\<And>nm i t' ts. i<size ts \<Longrightarrow> ts!i \<Rightarrow> t' \<Longrightarrow> P (ts!i) (t')
+    \<Longrightarrow> P (C nm  \<bullet>\<bullet> ts) (C nm \<bullet>\<bullet> ts[i:=t'])"
+  "\<And>t i t' ts. i<size ts \<Longrightarrow> ts!i \<Rightarrow> t' \<Longrightarrow> P (ts!i) (t')
+    \<Longrightarrow> P (\<Lambda> t \<bullet>\<bullet> ts) (\<Lambda> t \<bullet>\<bullet> ts[i:=t'])"
+  "\<And>v i t' ts. i<size ts \<Longrightarrow> ts!i \<Rightarrow> t' \<Longrightarrow> P (ts!i) (t')
+    \<Longrightarrow> P (term v  \<bullet>\<bullet> ts) (term v \<bullet>\<bullet> (ts[i:=t']))"
+shows "P t t'"
+proof-
+  { fix ts from assms have "P (t \<bullet>\<bullet> ts) (t' \<bullet>\<bullet> ts)"
+    proof(induct arbitrary: ts rule:Red_term.induct)
+      case term_C thus ?case by metis
+    next
+      case term_V thus ?case by metis
+    next
+      case term_Clo thus ?case by metis
+    next
+      case ctxt_Lam thus ?case by simp (metis foldl_Nil)
+    next
+      case (ctxt_At1 s s' t ts)
+      thus ?case using ctxt_At1(2)[of "t#ts"] by simp
+    next
+      case (ctxt_At2 t t' s ts)
+      { fix n rs assume "s = V n \<bullet>\<bullet> rs"
+	hence ?case using ctxt_At2(8)[of "size rs" "rs @ t # ts" t' n] ctxt_At2
+	  by simp (metis foldl_Nil)
+      } moreover
+      { fix nm rs assume "s = C nm \<bullet>\<bullet> rs"
+	hence ?case using ctxt_At2(9)[of "size rs" "rs @ t # ts" t' nm] ctxt_At2
+	  by simp (metis foldl_Nil)
+      } moreover
+      { fix r rs assume "s = \<Lambda> r \<bullet>\<bullet> rs"
+	hence ?case using ctxt_At2(10)[of "size rs" "rs @ t # ts" t'] ctxt_At2
+	  by simp (metis foldl_Nil)
+      } moreover
+      { fix v rs assume "s = term v \<bullet>\<bullet> rs"
+	hence ?case using ctxt_At2(11)[of "size rs" "rs @ t # ts" t'] ctxt_At2
+	  by simp (metis foldl_Nil)
+      } ultimately show ?case using tm_vector_cases[of s] by blast
+    qed
+  }
+  from this[of "[]"] show ?thesis by simp
+qed
+
+corollary Red_term_hnf_cases[consumes 1]:
+assumes "(t::tm) \<Rightarrow> t'"
+  "\<And>nm vs ts.
+  t = term (C\<^isub>U nm vs) \<bullet>\<bullet> ts \<Longrightarrow> t' = (C nm \<bullet>\<bullet> map term (rev vs)) \<bullet>\<bullet> ts \<Longrightarrow> P"
+  "\<And>x vs ts.
+  t = term (V\<^isub>U x vs) \<bullet>\<bullet> ts \<Longrightarrow> t' = (V x \<bullet>\<bullet> map term (rev vs)) \<bullet>\<bullet> ts \<Longrightarrow> P"
+  "\<And>vf vs n ts. t = term (Clo vf vs n) \<bullet>\<bullet> ts \<Longrightarrow>
+     t' = \<Lambda> (term (apply (lift 0 (Clo vf vs n)) (V\<^isub>U 0 []))) \<bullet>\<bullet> ts \<Longrightarrow> P"
+  "\<And>s s' ts. t = \<Lambda> s \<bullet>\<bullet> ts \<Longrightarrow> t' = \<Lambda> s' \<bullet>\<bullet> ts \<Longrightarrow> s \<Rightarrow> s' \<Longrightarrow> P"
+  "\<And>v v' ts. t = term v \<bullet>\<bullet> ts \<Longrightarrow> t' = term v' \<bullet>\<bullet> ts \<Longrightarrow> v \<Rightarrow> v' \<Longrightarrow> P"
+  "\<And>x i r' ts. i<size ts \<Longrightarrow> ts!i \<Rightarrow> r'
+    \<Longrightarrow> t = V x  \<bullet>\<bullet> ts \<Longrightarrow> t' = V x \<bullet>\<bullet> ts[i:=r'] \<Longrightarrow> P"
+  "\<And>nm i r' ts. i<size ts \<Longrightarrow> ts!i \<Rightarrow> r'
+    \<Longrightarrow> t = C nm  \<bullet>\<bullet> ts \<Longrightarrow> t' = C nm \<bullet>\<bullet> ts[i:=r'] \<Longrightarrow> P"
+  "\<And>s i r' ts. i<size ts \<Longrightarrow> ts!i \<Rightarrow> r'
+    \<Longrightarrow> t = \<Lambda> s \<bullet>\<bullet> ts \<Longrightarrow> t' = \<Lambda> s \<bullet>\<bullet> ts[i:=r'] \<Longrightarrow> P"
+  "\<And>v i r' ts. i<size ts \<Longrightarrow> ts!i \<Rightarrow> r'
+    \<Longrightarrow> t = term v  \<bullet>\<bullet> ts \<Longrightarrow> t' = term v \<bullet>\<bullet> (ts[i:=r']) \<Longrightarrow> P"
+shows "P" using assms
+apply -
+apply(induct rule:Red_term_hnf_induct)
+apply metis+
+done
+
+
+lemma [simp]: "C_normal(term v \<bullet>\<bullet> ts) \<longleftrightarrow> C_normal\<^bsub>ML\<^esub> v \<and> ts = []"
+by(fastsimp elim: C_normal.cases)
+
+lemma [simp]: "C_normal(\<Lambda> t \<bullet>\<bullet> ts) \<longleftrightarrow> C_normal t \<and> ts = []"
+by(fastsimp elim: C_normal.cases)
+
+lemma [simp]: "C_normal(C nm \<bullet>\<bullet> ts) \<longleftrightarrow>
+  (\<forall>t\<in>set ts. C_normal t) \<and> no_match_R nm (map dterm ts)"
+by(fastsimp elim: C_normal.cases)
+
+lemma [simp]: "C_normal(V x \<bullet>\<bullet> ts) \<longleftrightarrow> (\<forall>t \<in> set ts. C_normal t)"
+by(fastsimp elim: C_normal.cases)
+
+lemma no_match_ML_lift:
+  "no_match\<^bsub>ML\<^esub> ps vs \<longrightarrow> no_match\<^bsub>ML\<^esub> ps (map (lift k) vs)"
+apply(induct ps vs rule:no_match_ML.induct)
+apply simp
+apply(subst (1 2) no_match_ML.simps)
+apply clarsimp
+apply(rule_tac x=i in exI)
+apply simp
+apply(rule_tac x=nm' in exI)
+apply(rule_tac x="map (lift k) vs'" in exI)
+apply (fastsimp simp:rev_nth)
+done
+
+lemma no_match_compR_lift:
+  "no_match_compR nm vs \<Longrightarrow> no_match_compR nm (map (lift k) vs)"
+by (fastsimp simp: no_match_ML_lift)
+
+lemma [simp]: "C_normal\<^bsub>ML\<^esub> v \<Longrightarrow> C_normal\<^bsub>ML\<^esub>(lift k v)"
+apply(induct v arbitrary:k rule:lift_ml.induct)
+apply(simp_all add:no_match_compR_lift)
+done
+
+declare [[simp_depth_limit = 10]]
+
+lemma Red_term_pres_no_match:
+  "\<lbrakk>i < length ts; ts ! i \<Rightarrow> t'; no_match ps dts; dts = (map dterm ts)\<rbrakk>
+   \<Longrightarrow> no_match ps (map dterm (ts[i := t']))"
+proof(induct ps dts arbitrary: ts i t' rule:no_match.induct)
+  case (1 ps dts ts i t')
+  from `no_match ps dts` `dts = map dterm ts`
+  obtain j nm nm' rs rs' where ob: "j < size ts" "j < size ps"
+    "ps!j = C nm \<bullet>\<bullet> rs" "dterm (ts!j) = C nm' \<bullet>\<bullet> rs'"
+    "nm = nm' \<longrightarrow> no_match rs rs'"
+    by (subst (asm) no_match.simps) fastsimp
+  show ?case
+  proof (subst no_match.simps)
+    show "\<exists>k<min (length (map dterm (ts[i := t']))) (length ps).
+       \<exists>nm nm' rs rs'. ps!k  = C nm \<bullet>\<bullet> rs \<and>
+         map dterm (ts[i := t']) ! k = C nm' \<bullet>\<bullet> rs' \<and>
+        (nm = nm' \<longrightarrow> no_match rs rs')"
+      (is "\<exists>k < ?m. ?P k")
+    proof-
+      { assume [simp]: "j=i"
+        have "\<exists>rs'. dterm t' = C nm' \<bullet>\<bullet> rs' \<and> (nm = nm' \<longrightarrow> no_match rs rs')"
+	  using `ts ! i \<Rightarrow> t'`
+	proof(cases rule:Red_term_hnf_cases)
+	  case (5 v v' ts'')
+	  then obtain vs where [simp]:
+	    "v = C\<^isub>U nm' vs" "rs' = map dterm\<^bsub>ML\<^esub> (rev vs) @ map dterm ts''"
+	    using ob by(cases v) auto
+	  obtain vs' where [simp]: "v' = C\<^isub>U nm' vs'" "vs \<Rightarrow> vs'"
+	    using `v\<Rightarrow>v'` by(rule Red_ml.cases) auto
+	  obtain v' k where [arith]: "k<size vs" and "vs!k \<Rightarrow> v'"
+	    and [simp]: "vs' = vs[k := v']"
+	    using Red_ml_list_nth[OF `vs\<Rightarrow>vs'`] by fastsimp
+	  show ?thesis (is "\<exists>rs'. ?P rs' \<and> ?Q rs'")
+	  proof
+	    let ?rs' = "map dterm ((map term (rev vs) @ ts'')[(size vs - k - 1):=term v'])"
+	    have "?P ?rs'" using ob 5
+	      by(simp add: list_update_append map_update[symmetric] rev_update)
+	    moreover have "?Q ?rs'"
+	      apply rule
+	      apply(rule "1.hyps"[OF _ ob(3)])
+	      using "1.prems" 5 ob
+	      apply (auto simp:nth_append rev_nth ctxt_term[OF `vs!k \<Rightarrow> v'`])
+	      done
+	    ultimately show "?P ?rs' \<and> ?Q ?rs'" ..
+	  qed
+	next
+	  case (7 nm'' k r' ts'')
+	  show ?thesis (is "\<exists>rs'. ?P rs'")
+	  proof
+	    show "?P(map dterm (ts''[k := r']))"
+	      using 7 ob
+	      apply clarsimp
+	      apply(rule "1.hyps"[OF _ ob(3)])
+	      using 7 "1.prems" ob apply auto
+	      done
+	  qed
+	next
+	  case (9 v k r' ts'')
+	  then obtain vs where [simp]: "v = C\<^isub>U nm' vs" "rs' = map dterm\<^bsub>ML\<^esub> (rev vs) @ map dterm ts''"
+	    using ob by(cases v) auto
+	  show ?thesis (is "\<exists>rs'. ?P rs' \<and> ?Q rs'")
+	  proof
+	    let ?rs' = "map dterm ((map term (rev vs) @ ts'')[k+size vs:=r'])"
+	    have "?P ?rs'" using ob 9 by (auto simp: list_update_append)
+	    moreover have "?Q ?rs'"
+	      apply rule
+	      apply(rule "1.hyps"[OF _ ob(3)])
+	      using 9 "1.prems" ob by (auto simp:nth_append)
+	    ultimately show "?P ?rs' \<and> ?Q ?rs'" ..
+	  qed
+	qed (insert ob, auto)
+      }
+      hence "\<exists>rs'. dterm (ts[i := t'] ! j) = C nm' \<bullet>\<bullet> rs' \<and> (nm = nm' \<longrightarrow> no_match rs rs')"
+	using `i < size ts` ob by(simp add:nth_list_update)
+      hence "?P j" using prems by auto
+      moreover have "j < ?m" using `j < length ts` `j < size ps` by simp
+      ultimately show ?thesis by blast
+    qed
+  qed
+qed
+
+declare [[simp_depth_limit = 50]]
+
+lemma listsimps_eq_0_iff: "listsum ns = (0::nat) \<longleftrightarrow> (\<forall> n \<in> set ns. n = 0)"
+by(metis listsum sum_eq_0_conv)
+
+(* Generalize to suitable type class? *)
+lemma elem_le_listsum_nat: "k<size ns \<Longrightarrow> ns!k <= listsum(ns::nat list)"
+apply(induct ns arbitrary: k)
+apply(auto simp:nth_Cons')
+apply(metis diff_less less_imp_diff_less nat_neq_iff not_less_eq trans_le_add2)
+done
+
+lemma listsum_update: "k<size ns \<Longrightarrow>
+  listsum (ns[k := (n::nat)]) = listsum ns + n - ns!k"
+apply(induct ns arbitrary:k)
+apply (auto split:nat.split)
+apply(drule elem_le_listsum_nat)
+apply arith
+done
+(*
+lemma lem: "finite A \<Longrightarrow>
+  (\<Sum>x\<in>A. if P x then f x else g x) =
+  setsum f {a:A. P a} + setsum g {a:A. ~P a}"
+*)
+
+lemma Red_term_pres_no_match_it:
+  "\<lbrakk> \<forall> i < length ts. (ts ! i, ts' ! i) : Red_term ^^ (ns!i);
+    size ts' = size ts; size ns = size ts;
+    no_match ps (map dterm ts)\<rbrakk>
+   \<Longrightarrow> no_match ps (map dterm ts')"
+proof(induct n \<equiv> "listsum ns" arbitrary: ts ns)
+  case 0
+  hence "\<forall>i < size ts. ns!i = 0" by (simp add:listsimps_eq_0_iff)
+  with 0 show ?case by simp (metis nth_equalityI)
+next
+  case (Suc n)
+  then have "listsum ns \<noteq> 0" by arith
+  then obtain k l where "k<size ts" and [simp]: "ns!k = Suc l"
+    by(simp add:listsimps_eq_0_iff)
+      (metis Suc(4) gr0_implies_Suc in_set_conv_nth)
+  let ?ns = "ns[k := l]"
+  have "n = listsum ?ns" using Suc(6) `k<size ts` `size ns = size ts`
+    by (simp add:listsum_update)
+  obtain t' where "ts!k \<Rightarrow> t'" "(t', ts'!k) : Red_term^^l"
+    using Suc(2) `k<size ts` `size ns = size ts` `ns!k = Suc l`
+    by (metis rel_pow_Suc_E2)
+  then have 1: "\<forall>i<size(ts[k:=t']). (ts[k:=t']!i, ts'!i) : Red_term^^(?ns!i)"
+    using Suc(2) `k<size ts` `size ns = size ts`
+    by (auto simp add:nth_list_update)
+  note nm1 = Red_term_pres_no_match[OF `k<size ts` `ts!k \<Rightarrow> t'` Suc(5)]
+  show ?case by(rule Suc(1)[OF 1 _ _ nm1 `n = listsum ?ns`])
+               (simp_all add: `size ts' = size ts` `size ns = size ts`)
+qed
+
+
+lemma Red_term_pres_no_match_star:
+assumes "\<forall>i < length(ts::tm list). ts ! i \<Rightarrow>* ts' ! i" and "size ts' = size ts"
+    and "no_match ps (map dterm ts)"
+shows "no_match ps (map dterm ts')"
+proof-
+  let ?P = "%ns. size ns = size ts \<and>
+   (\<forall>i < length ts.(ts!i, ts'!i) : Red_term^^(ns!i))"
+  have "\<exists>ns. ?P ns" using assms(1)
+    by(subst Skolem_list_nth[symmetric])
+      (simp add:rtrancl_power)
+  from someI_ex[OF this] show ?thesis
+    by(fast intro: Red_term_pres_no_match_it[OF _ assms(2) _ assms(3)])
+qed
+
+lemma not_pure_term[simp]: "\<not> pure(term v)"
+proof
+  assume "pure(term v)" thus False
+  proof cases qed auto
+qed
+
+abbreviation RedMLs :: "tm list \<Rightarrow> tm list \<Rightarrow> bool" (infix "[\<Rightarrow>*]" 50) where
+"ss [\<Rightarrow>*] ts  \<equiv>  size ss = size ts \<and> (\<forall>i<size ss. ss!i \<Rightarrow>* ts!i)"
+
+
+fun C_U_args :: "tm \<Rightarrow> tm list" ("C\<^isub>U'_args") where
+"C\<^isub>U_args(s \<bullet> t) = C\<^isub>U_args s @ [t]" |
+"C\<^isub>U_args(term(C\<^isub>U nm vs)) = map term (rev vs)" |
+"C\<^isub>U_args _ = []"
+
+lemma [simp]: "C\<^isub>U_args(C nm \<bullet>\<bullet> ts) = ts"
+by (induct ts rule:rev_induct) auto
+
+lemma redts_term_cong: "v \<Rightarrow>* v' \<Longrightarrow> term v \<Rightarrow>* term v'"
+apply(erule converse_rtrancl_induct)
+apply(rule rtrancl_refl)
+apply(fast intro: converse_rtrancl_into_rtrancl dest: ctxt_term)
+done
+
+lemma C_Red_term_ML:
+  "v \<Rightarrow> v' \<Longrightarrow> C_normal\<^bsub>ML\<^esub> v \<Longrightarrow> dterm\<^bsub>ML\<^esub> v = C nm \<bullet>\<bullet> ts
+   \<Longrightarrow> dterm\<^bsub>ML\<^esub> v' = C nm \<bullet>\<bullet> map dterm (C\<^isub>U_args(term v')) \<and>
+      (\<forall>t\<in>set(C\<^isub>U_args(term v)). C_normal t) \<and>
+      C\<^isub>U_args(term v) [\<Rightarrow>*] C\<^isub>U_args(term v') \<and>
+      ts = map dterm (C\<^isub>U_args(term v))" and
+  "(vs:: ml list) \<Rightarrow> vs' \<Longrightarrow> i < length vs \<Longrightarrow> vs ! i \<Rightarrow>* vs' ! i"
+apply(induct arbitrary: nm ts and i rule:Red_ml_Red_ml_list.inducts)
+apply(simp_all add:Red_ml_list_length)
+  apply(frule Red_ml_list_length)
+  apply(simp add: redts_term_cong rev_nth)
+ apply(simp add:nth_Cons' r_into_rtrancl)
+apply(simp add:nth_Cons')
+done
+
+lemma C_redt: "t \<Rightarrow> t' \<Longrightarrow> C_normal t \<Longrightarrow> 
+    C_normal t' \<and> (dterm t = C nm \<bullet>\<bullet> ts \<longrightarrow>
+    (\<exists>ts'. ts' = map dterm (C\<^isub>U_args t') \<and> dterm t' = C nm \<bullet>\<bullet> ts' &
+     (\<forall>t\<in>set(C\<^isub>U_args t). C_normal t) \<and>
+     C\<^isub>U_args t [\<Rightarrow>*] C\<^isub>U_args t' \<and> ts = map dterm (C\<^isub>U_args t)))"
+apply(induct arbitrary: ts nm rule:Red_term_hnf_induct)
+apply simp_all
+apply (metis no_match_R_coincide rev_rev_ident)
+apply clarsimp
+apply rule
+apply (metis C_normal_ML_inv)
+apply clarify
+apply(drule (2) C_Red_term_ML)
+apply clarsimp
+apply clarsimp
+apply (metis List.set.simps(2) insert_code mem_def predicate1D set_update_subset_insert)
+apply clarsimp
+apply(rule)
+apply (metis List.set.simps(2) insert_code mem_def predicate1D set_update_subset_insert)
+apply rule
+apply clarify
+apply(drule bspec, assumption)
+apply simp
+apply(subst no_match.simps)
+apply(subst (asm) no_match.simps)
+apply clarsimp
+apply(rename_tac j nm nm' rs rs')
+apply(rule_tac x=j in exI)
+apply simp
+apply(case_tac "i=j")
+apply simp
+apply(rule_tac x=nm' in exI)
+apply(erule_tac x=rs' in meta_allE)
+apply(erule_tac x=nm' in meta_allE)
+apply clarsimp
+apply(metis Red_term_pres_no_match_star)
+apply (auto simp:nth_list_update)
+done
+
+
+lemma C_redts: "t \<Rightarrow>* t' \<Longrightarrow> C_normal t \<Longrightarrow>
+    C_normal t' \<and> (dterm t = C nm \<bullet>\<bullet> ts \<longrightarrow>
+    (\<exists>ts'. dterm t' = C nm \<bullet>\<bullet> ts' \<and>
+     (\<forall>t\<in>set(C\<^isub>U_args t). C_normal t) \<and> C\<^isub>U_args t [\<Rightarrow>*] C\<^isub>U_args t' \<and>
+     ts' = map dterm (C\<^isub>U_args t') \<and> ts = map dterm (C\<^isub>U_args t)))"
+apply(induct arbitrary: nm ts rule:converse_rtrancl_induct)
+apply simp
+using tm_vector_cases[of t']
+apply(elim disjE)
+apply clarsimp
+apply clarsimp
+apply clarsimp
+apply clarsimp
+apply(case_tac v)
+apply simp
+apply simp
+apply simp
+apply simp
+apply clarsimp
+apply (simp add:map_compose[symmetric])
+apply (simp add:map_compose[symmetric])
+apply simp
+apply simp
+apply(frule_tac nm=nm and ts="ts" in C_redt)
+apply assumption
+apply clarify
+apply rule
+apply metis
+apply clarify
+apply simp
+apply rule
+apply metis
+apply simp
+apply (metis rtrancl_trans)
+done
+
+lemma no_match_preserved:
+  "\<forall>t\<in>set ts. C_normal t \<Longrightarrow> ts [\<Rightarrow>*] ts'
+   \<Longrightarrow> no_match ps os \<Longrightarrow> os = map dterm ts \<Longrightarrow> no_match ps (map dterm ts')"
+proof(induct ps os arbitrary: ts ts' rule: no_match.induct)
+  case (1 ps os)
+  obtain i nm nm' ps' os' where "ps!i = C nm  \<bullet>\<bullet> ps'" "i < size ps" "i < size os" "os!i = C nm' \<bullet>\<bullet> os'" "nm=nm' \<longrightarrow> no_match ps' os'"
+    using 1(4) no_match.simps[of ps os] by fastsimp
+  note 1(5)[simp]
+  have "C_normal (ts ! i)" using 1(2) `i < size os` by auto
+  have "ts!i \<Rightarrow>* ts'!i" using 1(3) `i < size os` by auto
+  have "dterm (ts ! i) = C nm' \<bullet>\<bullet> os'" using `os!i = C nm' \<bullet>\<bullet> os'` `i < size os`
+    by (simp add:nth_map)
+  from C_redts [OF `ts!i \<Rightarrow>* ts'!i` `C_normal (ts!i)`] this obtain ss' rs rs' :: "tm list"
+    where "\<forall>t\<in>set rs. C_normal t" 
+    "dterm (ts' ! i) = C nm' \<bullet>\<bullet> ss'" "length rs = length rs'"
+    "\<forall>i<length rs. rs ! i \<Rightarrow>* rs' ! i" "ss' = map dterm rs'" "os' = map dterm rs"
+    by fastsimp
+  show ?case
+    apply(subst no_match.simps)
+    apply(rule_tac x=i in exI)
+    using prems
+    apply clarsimp
+    apply(rule 1(1)[of i nm' _ nm' "map dterm rs" rs])
+    apply simp_all
+    done
+qed
+
+lemma Lam_Red_term_itE:
+  "(\<Lambda> t, t') : Red_term^^i \<Longrightarrow> \<exists>t''. t' = \<Lambda> t'' \<and> (t,t'') : Red_term^^i"
+apply(induct i arbitrary: t')apply simp
+apply(erule rel_pow_Suc_E)
+apply(erule Red_term.cases)
+apply (simp_all)
+apply blast+
+done
+
+
+lemma Red_term_it: "(V x \<bullet>\<bullet> rs, r) : Red_term^^i
+  \<Longrightarrow> \<exists>ts is. r = V x \<bullet>\<bullet> ts \<and> size ts = size rs & size is = size rs \<and>
+       (\<forall>j<size ts. (rs!j, ts!j) : Red_term^^(is!j) \<and> is!j <= i)"
+proof(induct i arbitrary:rs)
+  case 0
+  moreover
+  have "\<exists>is. length is = length rs \<and>
+   (\<forall>j<size rs. (rs!j, rs!j) \<in> Red_term ^^ is!j \<and> is!j = 0)" (is "\<exists>is. ?P is")
+  proof
+    show "?P(replicate (size rs) 0)" by simp
+  qed
+  ultimately show ?case by auto
+next
+  case (Suc i rs)
+  from `(V x \<bullet>\<bullet> rs, r) \<in> Red_term ^^ Suc i`
+  obtain r' where r': "V x \<bullet>\<bullet> rs \<Rightarrow> r'" and "(r',r) \<in> Red_term ^^ i"
+    by (metis rel_pow_Suc_D2)
+  from r' have "\<exists>k<size rs. \<exists>s. rs!k \<Rightarrow> s \<and> r' = V x \<bullet>\<bullet> rs[k:=s]"
+  proof(induct rs arbitrary: r' rule:rev_induct)
+    case Nil thus ?case by(fastsimp elim: Red_term.cases)
+  next
+    case (snoc r rs)
+    hence "(V x \<bullet>\<bullet> rs) \<bullet> r \<Rightarrow> r'" by simp
+    thus ?case
+    proof(cases rule:Red_term.cases)
+      case (ctxt_At1 s s' t)
+      then obtain k s'' where "k<length rs" "rs ! k \<Rightarrow> s''" "s' = V x \<bullet>\<bullet> rs[k := s'']"
+	using snoc(1) by force
+      then show ?thesis (is "\<exists>k < ?n. \<exists>s. ?P k s")
+      proof-
+	have "k<?n \<and> ?P k s''" using prems
+	  by (simp add:nth_append) (metis last_snoc butlast_snoc list_update_append1)
+	thus ?thesis by blast
+      qed
+    next
+      case (ctxt_At2 t t' s)
+      then show ?thesis (is "\<exists>k < ?n. \<exists>s. ?P k s")
+      proof-
+	have "size rs<?n \<and> ?P (size rs) t'" using prems by simp
+	thus ?thesis by blast
+      qed
+    qed auto
+  qed
+  then obtain k s where "k<size rs" "rs!k \<Rightarrow> s" and [simp]: "r' = V x \<bullet>\<bullet> rs[k:=s]" by metis
+  from Suc(1)[of "rs[k:=s]"] `(r',r) \<in> Red_term ^^ i`
+  show ?case using `k<size rs` `rs!k \<Rightarrow> s`
+    apply auto
+    apply(rule_tac x="is[k := Suc(is!k)]" in exI)
+    apply (auto simp:nth_list_update)
+    apply(erule_tac x=k in allE)
+    apply auto
+    apply (metis rel_pow_Suc_I2 relpow.simps(2))
+    done
+qed
+
+lemma C_Red_term_it:  "(C nm \<bullet>\<bullet> rs, r) : Red_term^^i
+  \<Longrightarrow> \<exists>ts is. r = C nm \<bullet>\<bullet> ts \<and> size ts = size rs \<and> size is = size rs \<and>
+        (\<forall>j<size ts. (rs!j, ts!j) \<in> Red_term^^(is!j) \<and> is!j \<le> i)"
+proof(induct i arbitrary:rs)
+  case 0
+  moreover
+  have "\<exists>is. length is = length rs \<and>
+   (\<forall>j<size rs. (rs!j, rs!j) \<in> Red_term ^^ is!j \<and> is!j = 0)" (is "\<exists>is. ?P is")
+  proof
+    show "?P(replicate (size rs) 0)" by simp
+  qed
+  ultimately show ?case by auto
+next
+  case (Suc i rs)
+  from `(C nm \<bullet>\<bullet> rs, r) \<in> Red_term ^^ Suc i`
+  obtain r' where r': "C nm \<bullet>\<bullet> rs \<Rightarrow> r'" and "(r',r) \<in> Red_term ^^ i"
+    by (metis rel_pow_Suc_D2)
+  from r' have "\<exists>k<size rs. \<exists>s. rs!k \<Rightarrow> s \<and> r' = C nm \<bullet>\<bullet> rs[k:=s]"
+  proof(induct rs arbitrary: r' rule:rev_induct)
+    case Nil thus ?case by(fastsimp elim: Red_term.cases)
+  next
+    case (snoc r rs)
+    hence "(C nm \<bullet>\<bullet> rs) \<bullet> r \<Rightarrow> r'" by simp
+    thus ?case
+    proof(cases rule:Red_term.cases)
+      case (ctxt_At1 s s' t)
+      then obtain k s'' where "k<length rs" "rs ! k \<Rightarrow> s''" "s' = C nm \<bullet>\<bullet> rs[k := s'']"
+	using snoc(1) by force
+      then show ?thesis (is "\<exists>k < ?n. \<exists>s. ?P k s")
+      proof-
+	have "k<?n \<and> ?P k s''" using prems
+	  by (simp add:nth_append) (metis last_snoc butlast_snoc list_update_append1)
+	thus ?thesis by blast
+      qed
+    next
+      case (ctxt_At2 t t' s)
+      then show ?thesis (is "\<exists>k < ?n. \<exists>s. ?P k s")
+      proof-
+	have "size rs<?n \<and> ?P (size rs) t'" using prems by simp
+	thus ?thesis by blast
+      qed
+    qed auto
+  qed
+  then obtain k s where "k<size rs" "rs!k \<Rightarrow> s" and [simp]: "r' = C nm \<bullet>\<bullet> rs[k:=s]" by metis
+  from Suc(1)[of "rs[k:=s]"] `(r',r) \<in> Red_term ^^ i`
+  show ?case using `k<size rs` `rs!k \<Rightarrow> s`
+    apply auto
+    apply(rule_tac x="is[k := Suc(is!k)]" in exI)
+    apply (auto simp:nth_list_update)
+    apply(erule_tac x=k in allE)
+    apply auto
+    apply (metis rel_pow_Suc_I2 relpow.simps(2))
+    done
+qed
+
+
+lemma pure_At[simp]: "pure(s \<bullet> t) \<longleftrightarrow> pure s \<and> pure t"
+by(fastsimp elim: pure.cases)
+
+lemma pure_foldl_At[simp]: "pure(s \<bullet>\<bullet> ts) \<longleftrightarrow> pure s \<and> (\<forall>t\<in>set ts. pure t)"
+by(induct ts arbitrary: s) auto
+
+lemma nbe_C_normal_ML:
+assumes "term v \<Rightarrow>* t'" "C_normal\<^bsub>ML\<^esub> v" "pure t'" shows "normal t'"
+proof -
+  { fix t t' i v
+    assume "(t,t') : Red_term^^i"
+    hence "t = term v \<Longrightarrow> C_normal\<^bsub>ML\<^esub> v \<Longrightarrow> pure t' \<Longrightarrow> normal t'"
+    proof(induct i arbitrary: t t' v rule:less_induct)
+    case (less k)
+    show ?case
+    proof (cases k)
+      case 0 thus ?thesis using less by auto
+    next
+      case (Suc i)
+      then obtain i' s where "t \<Rightarrow> s" "(s,t') : Red_term^^i'" and [arith]: "i' <= i"
+	by (metis eq_imp_le less(5) Suc rel_pow_Suc_D2)
+      hence "term v \<Rightarrow> s" using Suc less by simp
+      thus ?thesis
+      proof cases
+	case (term_C nm vs)
+	have 0:"no_match_compR nm vs" using prems by auto
+	let ?n = "size vs"
+	have 1: "(C nm \<bullet>\<bullet> map term (rev vs),t') : Red_term^^i'"
+	  using term_C `(s,t') : Red_term^^i'` by simp
+	with C_Red_term_it[OF 1] 
+	obtain ts ks where [simp]: "t' = C nm \<bullet>\<bullet> ts"
+	  and sz: "size ts = ?n \<and> size ks = ?n \<and>
+	  (\<forall>i<?n. (term((rev vs)!i), ts!i) : Red_term^^(ks!i) \<and> ks ! i \<le> i')"
+	  by(auto cong:conj_cong)
+	have pure_ts: "\<forall>t\<in>set ts. pure t" using `pure t'` by simp
+	{ fix i assume "i<size vs"
+	  moreover hence "(term((rev vs)!i), ts!i) : Red_term^^(ks!i)" by(metis sz)
+	  ultimately have "normal (ts!i)"
+	    apply -
+	    apply(rule less(1))
+	    prefer 5 apply assumption
+	    using sz Suc apply fastsimp
+	    apply(rule refl)
+	    using less term_C
+	    apply(auto)
+	    apply (metis in_set_conv_nth length_rev set_rev)
+	    apply (metis in_set_conv_nth pure_ts sz)
+	    done
+	} note 2 = this
+	have 3: "no_match_R nm (map dterm (map term (rev vs)))"
+	  apply(subst map_dterm_term)
+	  apply(rule no_match_R_coincide) using 0 by simp
+	have 4: "map term (rev vs) [\<Rightarrow>*] ts"
+	proof -
+          have "(C nm \<bullet>\<bullet> map term (rev vs),t'): Red_term^^i'" using prems by auto
+	  from C_Red_term_it[OF this] obtain ts' "is"
+	    where "t' = C nm  \<bullet>\<bullet> ts'"  "length ts' = ?n \<and> length is =?n \<and>
+           (\<forall>j< ?n. (map term (rev vs) ! j, ts' ! j) \<in> Red_term ^^ is ! j \<and> is ! j \<le> i')"
+	    using prems by auto
+          from `t' = C nm \<bullet>\<bullet> ts'` `t' = C nm \<bullet>\<bullet> ts` have "ts = ts'" by simp
+	  show ?thesis using prems by (auto  simp: rtrancl_is_UN_rel_pow)
+	qed
+	have 5: "\<forall>t\<in>set(map term vs). C_normal t"  using prems by auto
+        have "no_match_R nm (map dterm ts)"
+	  apply auto
+	  apply(subgoal_tac "no_match aa (map dterm (map term (rev vs)))")
+	  prefer 2
+	  using 3 apply blast 
+          using 4 5 no_match_preserved[OF _ _ _ refl, of "map term (rev vs)" "ts"] by simp
+	hence 6: "no_match_R nm ts" by(metis map_dterm_pure[OF pure_ts])
+	then show "normal t'"
+	  apply(simp)
+	  apply(rule normal.intros(3))
+	  using 2 sz apply(fastsimp simp:set_conv_nth)
+	  apply auto
+	  apply(subgoal_tac "no_match aa (take (size aa) ts)")
+	  apply (metis no_match)
+	  apply(fastsimp intro:no_match_take)
+	  done
+      next
+	case (term_V x vs)
+	let ?n = "size vs"
+	have 1: "(V x \<bullet>\<bullet> map term (rev vs),t') : Red_term^^i'" using term_V `(s,t') : Red_term^^i'` by simp
+	with Red_term_it[OF 1] obtain ts "is" where [simp]: "t' = V x \<bullet>\<bullet> ts" and 2: "length ts = ?n \<and>
+          length is = ?n \<and> (\<forall>j<?n. (term (rev vs ! j), ts ! j) \<in> Red_term ^^ is ! j \<and> is ! j \<le> i')"
+	  by (auto cong:conj_cong)
+	have "\<forall>j<?n. normal(ts!j)"
+	proof(clarify)
+	  fix j assume 0: "j < ?n"
+	  then have "is!j < k" using `k=Suc i` 2 by auto
+	  have red: "(term (rev vs ! j), ts ! j) \<in> Red_term ^^ is ! j" using `j < ?n` 2 by auto
+	  have pure: "pure (ts ! j)" using `pure t'` 0 2 by auto
+	  have Cnm: "C_normal\<^bsub>ML\<^esub> (rev vs ! j)" using less term_V by simp (metis 0 in_set_conv_nth length_rev set_rev)
+	  from less(1)[OF `is!j < k` refl Cnm pure red] show "normal(ts!j)" .
+	qed
+	note 3=this
+	show ?thesis by simp (metis normal.intros(1) in_set_conv_nth 2 3)
+      next
+	case (term_Clo f vs n)
+	let ?u = "apply (lift 0 (Clo f vs n)) (V\<^isub>U 0 [])"
+	from term_Clo `(s,t') : Red_term^^i'`
+	obtain t'' where [simp]: "t' = \<Lambda> t''" and 1: "(term ?u, t'') : Red_term^^i'" by(metis Lam_Red_term_itE)
+	have "i' < k" using `k = Suc i` by arith
+	have "pure t''" using `pure t'` by simp
+	have "C_normal\<^bsub>ML\<^esub> ?u" using less term_Clo by(simp)
+	from less(1)[OF `i' < k` refl `C_normal\<^bsub>ML\<^esub> ?u` `pure t''` 1] show ?thesis by(simp add:normal.intros)
+      next
+	case (ctxt_term u u')
+	have "i' < k" using `k = Suc i` by arith
+	have "C_normal\<^bsub>ML\<^esub> u'" by (metis C_normal_ML_inv ctxt_term less tm.simps(25))
+	have "(term u', t') \<in> Red_term ^^ i'" using prems by auto
+	from less(1)[OF `i' < k` refl `C_normal\<^bsub>ML\<^esub> u'` `pure t'` this] show ?thesis .
+      qed auto
+    qed
+  qed
+  }
+  thus ?thesis using assms(2-) rtrancl_imp_rel_pow[OF assms(1)] by blast
+qed
+
+lemma C_normal_ML_compile:
+  "pure t \<Longrightarrow> \<forall>i. C_normal\<^bsub>ML\<^esub>(\<sigma> i) \<Longrightarrow> C_normal\<^bsub>ML\<^esub> (compile t \<sigma>)"
+by(induct t arbitrary: \<sigma>) (simp_all add: C_normal_ML_lift_ML)
+
+corollary nbe_normal:
+  "pure t \<Longrightarrow> term(comp_fixed t) \<Rightarrow>* t' \<Longrightarrow> pure t' \<Longrightarrow> normal t'"
+apply(erule nbe_C_normal_ML)
+apply(simp add: C_normal_ML_compile)
+apply assumption
+done
+
 (*<*)
 end
 (*>*)
